Ticket lock passing

src/example/TicketLock.v
@@ -5,7 +5,7 @@ From Fairness Require Import pind Axioms ITreeLib Red TRed IRed2 WFLibLarge.
 From Fairness Require Import FairBeh Mod Linking.
 From Fairness Require Import PCM IProp IPM IPropAux.
 From Fairness Require Import IndexedInvariants OpticsInterp SimWeakest.
-From Fairness Require Import TemporalLogic SCMemSpec LifetimeRA TicketLockRA.
+From Fairness Require Import TemporalLogic SCMemSpec OneShotsRA TicketLockRA AuthExclsRA.
 
 Module TicketLock.
 
@@ -44,21 +44,6 @@ Module TicketLock.
         trigger Yield
     .
 
-    (** TODO : more rules for module composition. *)
-    (* Definition omod : Mod.t := *)
-    (*   Mod.mk *)
-    (*     (* tt *) *)
-    (*     (Mod.st_init Client) *)
-    (*     (Mod.get_funs [("lock", Mod.wrap_fun lock); *)
-    (*                    ("unlock", Mod.wrap_fun unlock)]) *)
-    (* . *)
-
-    (* Definition module gvs : Mod.t := *)
-    (*   OMod.close *)
-    (*     (omod) *)
-    (*     (SCMem.mod gvs) *)
-    (* . *)
-
   End TICKET.
 
 End TicketLock.
@@ -80,9 +65,10 @@ Section SPEC.
   Context {HasMEMRA: @GRA.inG memRA Γ}.
 
   Context {HasTicket : @GRA.inG TicketRA Γ}.
-  Context {HasShots : @GRA.inG ShotsRA Γ}.
+  Context {AuthExclAnys : @GRA.inG (AuthExcls.t (nat * nat * nat))%ra Γ}.
+  Context {HasOneShots : @GRA.inG (OneShots.t unit) Γ}.
 
-  Ltac red_tl_all := red_tl; red_tl_memra; red_tl_ticket.
+  Ltac red_tl_all := red_tl; red_tl_memra; red_tl_ticket; red_tl_authexcls; red_tl_oneshots.
 
   Lemma lock_loop_red own_loc my_tk :
     @TicketLock.lock_loop tgt_state tgt_ident (own_loc, my_tk)
@@ -97,75 +83,26 @@ Section SPEC.
   Qed.
 
   (** Invariants. *)
-  (* Ref: Lecture Notes on Iris. *)
-  (* Definition tklockInv (i : nat) (r sr: nat) (lo ln : SCMem.val) (P : sProp i) (l : nat)
-    : sProp (1+i) :=
-    (∃ (o n o_obl : τ{nat, 1+i}) (D : τ{gset nat, 1+i}),
-        (⤉ (lo ↦ o))
-          ∗ (⤉ (ln ↦ n))
-          ∗ (⤉ (s_ticket_black r o D))
-          ∗ (⤉ (s_shots_base sr n))
-          ∗ (⌜forall tk, (tk < n) <-> (tk ∈ D)⌝)
-          ∗ (((⤉ s_ticket_locked r o) ∗ (⤉P) ∗
-               ((⌜o = n⌝) ∨ (⌜o < n⌝ ∗ ∃ (tid obl: τ{nat, 1+i}) (ds : τ{ listT (nat * nat * Φ)%stype, 1+i }),
-                                        (⤉ Duty(tid) ((o_obl, 0, s_shots_shot sr o) :: ds))
-                                        ∗ (⤉ ○Duty(tid) ds)
-                                        ∗ ◇[o_obl](l, 4)
-                                        ∗ (⤉ s_ticket_wait r o tid obl)
-                                        ∗ (⤉ s_shots_pending sr o)
-                                        ∗ ◆[o_obl, l])))
-             ∨ (∃ (tid obl: τ{nat, 1+i}), ((⤉ s_ticket_issued r o tid obl)
-                ∗ (⤉ s_shots_pending sr o)
-                ∗ ◆[o_obl, l]
-                ∗ (⤉ -[o_obl](0)-◇ s_shots_shot sr o)))
-            )
-          ∗ ([∗ (1+i) set] tk ∈ D,
-              (⌜tk < o⌝ ∗ ∃ (tid obl : τ{nat}), (⤉ s_ticket_issued r (tk : nat) tid obl))
-              ∨ (⌜tk = o⌝)
-              ∨ (⌜tk > o⌝) ∗ (∃ (tid obl : τ{nat}) (ds : τ{ listT (nat * nat * Φ)%stype, 1+i}),
-                  (⤉ Duty(tid) ds)
-                  ∗ (⤉ ○Duty(tid) ds)
-                  ∗ (⤉ s_ticket_wait r tk tid obl)
-                  ∗ (⤉ s_shots_pending sr tk)
-                  ∗ (◇[obl](1 + l, tk - o))
-                  ∗ (o_obl -(0)-◇ obl))
-            )
-    )%S. *)
-
-    Definition tklockInv (i : nat) (γt γs: nat) (lo ln : SCMem.val) (P : sProp i) (l : nat)
-    : sProp i :=
-    (∃ (o n κu : τ{nat, i}) (D : τ{gset nat, i}),
-        (lo ↦ o)
-          ∗ (ln ↦ n)
-          ∗ (s_ticket_black γt o D)
-          ∗ (s_shots_base γs n)
-          ∗ ⌜forall tk, (tk < n) <-> (tk ∈ D)⌝
-          ∗ ((s_ticket_locked γt o ∗ P ∗
-               ((⌜o = n⌝) ∨ (⌜o < n⌝ ∗ ∃ (κack : τ{nat, i}),
-                                        (s_ticket_wait γt o κu κack)
-                                        ∗ (-[κu](0)-◇ s_shots_shot γs o κu)
-                                        ∗ (⋈ [κu])
-                                        ∗ (s_shots_pending γs o κu)
-                                        ∗ ◆[κu, l])))
-             ∨ (∃ (κack: τ{nat, i}),
-                (s_ticket_issued γt o κu κack)
-                ∗ (-[κu](0)-◇ s_shots_shot γs o κu)
-                ∗ (⋈ [κu])
-                ∗ (s_shots_pending γs o κu)
-                ∗ ◆[κu, l])
-            )
-          ∗ ([∗ i set] tk ∈ D,
-              (⌜tk < o⌝ ∗ ∃ (κu κack : τ{nat}), (s_ticket_issued γt (tk : nat) κu κack))
-              ∨ (⌜tk = o⌝)
-              ∨ (⌜tk > o⌝) ∗ (∃ (κu' κack' : τ{nat}),
-                  (-[κu'](0)-⧖ s_shots_shot γs tk κu')
-                  ∗ (⧖ [κu', (1/2)])
-                  ∗ (s_ticket_wait γt tk κu' κack')
-                  ∗ (s_shots_pending γs tk κu')
-                  ∗ (◇[κack'](1 + l, tk - o))
-                  ∗ (κu -(0)-◇ κack')
-                  ∗ ◆[κu', l])
-            )
+  Definition tklockInv (i : nat) (γt : nat) (lo ln : SCMem.val) (P : sProp i) (l b : nat) : sProp i :=
+    (∃ (o n κu γs pass : τ{nat, i}) (D : τ{gset nat, i}),
+      (lo ↦ o)
+      ∗ (ln ↦ n)
+      ∗ (s_ticket_black γt D)
+      ∗ ⌜forall tk, (o <= tk < n) <-> (tk ∈ D)⌝
+      ∗ ⌜pass <= b⌝
+      ∗ (● γt (κu, γs, pass))
+      ∗ ((⌜o = n⌝ ∗ (○ γt (κu, γs, pass)) ∗ P)
+        ∨ ◆[κu, l] ∗ (-[κu](0)-◇ ▿ γs tt) ∗ (⋈ [κu]) ∗ (△ γs 1) (* Promise to unlock *)
+          ∗ (∃ (κack : τ{nat, i}),
+              (s_ticket_wait γt o [κu; γs; κack; pass])
+              ∗ (s_ticket_issued γt o [κu; γs; κack; pass] ∨ (○ γt (κu, γs, pass) ∗ P))))
+      ∗ ([∗ i set] tk ∈ D,
+          ⌜tk = o⌝
+          ∨ ⌜tk > o⌝
+            ∗ (∃ (κu' κack' γs' : τ{nat}),
+              ◆[κu', l] ∗ (-[κu'](0)-⧖ ▿ γs' tt) ∗ ⧖ [κu', (1/2)] ∗ (△ γs' 1) (* Delayed promises to unlock *)
+              ∗ (s_ticket_wait γt tk [κu'; γs'; κack'; b])
+              ∗ (◇[κack'](1 + l, pass + (b + 1) * (tk - o))) ∗ (κu -(0)-◇ κack'))) (* Dependent obligations *)
     )%S.
 
   (* Namespace for TicketLock invariants. *)
@@ -174,13 +111,13 @@ Section SPEC.
   Lemma mask_disjoint_ticketlock_state_tgt : ↑N_TicketLock ## (↑N_state_tgt : coPset).
   Proof. apply ndot_ne_disjoint. ss. Qed.
 
-  Definition isTicketLock i (γt γs: nat) (v : SCMem.val * SCMem.val) (P : sProp i) (l : nat)
+  Definition isTicketLock i (γt : nat) (v : SCMem.val * SCMem.val) (P : sProp i) (l b : nat)
     : sProp i :=
     (∃ (lo ln : τ{SCMem.val}) (N : τ{namespace, i}),
         (⌜(↑N ⊆ (↑N_TicketLock : coPset))⌝)
-          ∗ (⌜0 < l⌝) ∗ (⌜v = (lo, ln)⌝) ∗ syn_inv i N (tklockInv i γt γs lo ln P l))%S.
+          ∗ (⌜0 < l⌝) ∗ (⌜v = (lo, ln)⌝) ∗ syn_inv i N (tklockInv i γt lo ln P l b))%S.
 
-  Global Instance isSpinlock_persistent i r or v P l : Persistent (⟦isTicketLock i r or v P l, i⟧).
+  Global Instance isSpinlock_persistent i γt v P l b : Persistent (⟦isTicketLock i γt v P l b, i⟧).
   Proof.
     unfold Persistent. iIntros "H". unfold isTicketLock.
     red_tl. iDestruct "H" as "[%lo H]". iExists lo.
@@ -190,26 +127,26 @@ Section SPEC.
   Qed.
 
   Lemma make_isTicketLock
-        i lo ln P l (LT : 0 < l)
+        i lo ln P l b (LT : 0 < l)
         Es
     :
     ⊢
-      ⟦((⤉ (lo ↦ 0)) ∗ (⤉ (ln ↦ 0)) ∗ (⤉ P) ∗ (⤉ s_ticket_auth) ∗ (⤉ s_shots_auth))%S, 1+i⟧
+      ⟦((⤉ (lo ↦ 0)) ∗ (⤉ (ln ↦ 0)) ∗ (⤉ P) ∗ (⤉ s_ticket_auth))%S, 1+i⟧
         -∗
-        ⟦(∃ (γr γs : τ{nat, 1+i}), =|1+i|={Es}=> (⤉ isTicketLock i γr γs (lo, ln) P l))%S, 1+i⟧.
+        ⟦(∃ (γt : τ{nat, 1+i}), =|1+i|={Es}=> (⤉ isTicketLock i γt (lo, ln) P l b))%S, 1+i⟧.
   Proof.
-    simpl. red_tl_all; simpl. iIntros "(LO & LN & P & TAUTH & OTAUTH)".
-    iPoseProof (TicketRA_alloc 0 with "TAUTH") as "(%r & ALLOC)". iExists r. red_tl; simpl.
-    iPoseProof (ShotsRA_alloc with "OTAUTH") as "(%sr & OALLOC)". iExists sr.
-    rewrite red_syn_fupd; simpl. iMod "ALLOC" as "(TAUTH & TB & TL)". iMod "OALLOC" as "(OAUTH & OBASE)".
-    iMod ((FUpd_alloc _ _ _ i (N_TicketLock)) (tklockInv i r sr lo ln P l) with "[-]") as "#TINV". auto.
-    { unfold tklockInv. simpl. red_tl. iExists 0. red_tl; simpl. iExists 0.
-      red_tl; simpl. iExists 0. red_tl; simpl. iExists ∅.
-      red_tl_all; simpl. iFrame. iSplit; auto.
-      (* iSplit. *)
-      { iPureIntro. split; i; inv H. }
+    simpl. red_tl_all; simpl. iIntros "(LO & LN & P & TAUTH)".
+    iPoseProof (TicketRA_alloc 0 0 b with "TAUTH") as "(%γt & ALLOC)". iExists γt.
+    rewrite red_syn_fupd; simpl. iMod "ALLOC" as "(TAUTH & TB & LB & LW)".
+    iMod ((FUpd_alloc _ _ _ i (N_TicketLock)) (tklockInv i γt lo ln P l b) with "[-]") as "#TINV". auto.
+    { unfold tklockInv. simpl. red_tl.
+      iExists 0. red_tl; simpl. iExists 0. red_tl; simpl.
+      iExists 0. red_tl; simpl. iExists 0. red_tl; simpl. iExists b; red_tl. iExists ∅. red_tl_all; simpl.
+      iFrame. iSplit; auto.
+      { iPureIntro. split; i; inv H. lia. }
+      iSplit; auto.
       iSplitL; cycle 1. auto.
-      iLeft. iSplitL "TL"; auto. iSplitL "P"; auto.
+      iLeft. iSplitR; auto. iFrame.
     }
     iModIntro.
     unfold isTicketLock. red_tl; simpl. iExists lo. red_tl; simpl. iExists ln. red_tl; simpl.
@@ -218,166 +155,123 @@ Section SPEC.
     iSplitL ""; try iPureIntro; auto.
   Qed.
 
-  Lemma TicketLock_lock_spec
-        tid i
-        (E : coPset)
-        (IN : ⊤ ⊆ E)
-    :
-    ⊢ ∀ γt γs lo ln (P : sProp i) l (ds : list (nat * nat * sProp i)),
-        [@ tid, i, E @]
-          ⧼⟦(((syn_tgt_interp_as i sndl (fun m => (s_memory_black m)))
-                ∗ (⤉ isTicketLock i γt γs (lo, ln) P l)
-                ∗ (⤉ (Duty(tid) ds))
-                ∗ ⤉ ◇{ds@1}(5 + l, 1))%S), 1+i⟧⧽
-            (OMod.close_itree Client (SCMem.mod gvs) (TicketLock.lock (lo, ln)))
-            ⧼rv, ⟦(∃ (o κu : τ{nat, 1+i}),
-                    (⤉ P)
-                    ∗ (⤉ s_ticket_locked γt o)
-                    ∗ (⤉ (Duty(tid) ((κu, 0, s_shots_shot γs o κu) :: ds)))
-                    ∗ ◇[κu](l, 1))%S, 1+i⟧⧽
+  Lemma TicketLock_lock_loop_spec
+        tid i N l
+        (NIN : ↑N ⊆ (↑N_TicketLock : coPset))
+        (LT : 0 < l)
+  :
+  ⊢ ∀ γt lo ln (P : sProp i) b n κu γs κack (ds : list (nat * nat * sProp i)),
+    [@ tid, i, ⊤ @]
+      ⧼⟦((⤉ syn_inv i N (tklockInv i γt lo ln P l b))
+        ∗ (syn_tgt_interp_as i sndl (fun m => s_memory_black m))
+        ∗ (⤉ Duty(tid)((κu, 0, ▿ γs tt) :: ds))
+        ∗ (◇{(ds@1)}(2, 1))
+        ∗ (⤉ ⦃◆[κack] & ◇{(ds@1)%S}(2)⦄)
+        ∗ (◇[κu](l, 2))
+        ∗ (⤉ s_ticket_issued γt n [κu; γs; κack; b]))%S, 1+i⟧⧽
+        (OMod.close_itree Client (SCMem.mod gvs) (TicketLock.lock_loop (lo, SCMem.val_nat n)))
+        ⧼rv, ⟦((⤉ Duty(tid)((κu, 0, ▿ γs tt) :: ds))
+            ∗ (⤉ ○ γt (κu, γs, b))
+            ∗ (⤉ P))%S, 1+i⟧⧽
   .
   Proof.
-    iIntros. iStartTriple. iIntros "PRE POST". unfold TicketLock.lock.
-    iApply wpsim_discard. apply IN.
-    unfold isTicketLock. iEval (red_tl_all; simpl; rewrite red_syn_tgt_interp_as) in "PRE".
-    iEval (red_tl_all; simpl) in "PRE".
-    iDestruct "PRE" as "(#MEM & PRE & DUTY & PCS)".
-    iDestruct "PRE" as (lo') "PRE". iEval (red_tl_all; simpl) in "PRE".
-    iDestruct "PRE" as (ln') "PRE". iEval (red_tl_all; simpl) in "PRE".
-    iDestruct "PRE" as (N) "PRE". iEval (red_tl_all; simpl; rewrite red_syn_inv) in "PRE".
-    iDestruct "PRE" as "(%SUB & %GT & %EQ & #TINV)". symmetry in EQ. clarify.
+    iIntros. iStartTriple. simpl. red_tl_all; simpl. rewrite red_syn_inv; rewrite red_syn_tgt_interp_as.
+    iIntros "(#INV & #MEM & DUTY & PCS & CCS & PC & ISSUED)". iIntros "POST".
 
-    (* YIELD *)
-    rred2r.
-    iMod (pcs_drop _ _ 1 _ (4+l) 3 with "[PCS]") as "PCS". 2:{ iFrame. } auto.
-    iMod (pcs_decr _ _ 1 _ with "PCS") as "[PCS' PCS]". auto.
-    iMod (pcs_drop _ _ 1 _ 1 4 with "PCS'") as "PCS'". lia.
-    iCombine "DUTY" "PCS'" as "DUTY".
-    iApply (wpsim_yieldR2 with "DUTY"). auto. auto.
-    iIntros "DUTY CRED PCS'".
+    iRevert "PCS DUTY PC ISSUED POST".
+    iMod (ccs_ind2 with "CCS [-]") as "IND".
+    2:{ iApply "IND". }
+    iModIntro. iExists 0. iIntros "IH". iModIntro. iIntros "PCS DUTY PC ISSUED POST".
+    iMod (pcs_drop _ _ 1 _ _ 2 with "[PCS]") as "PCS". 2:{ iFrame. } auto.
 
-    (* OPEN *)
-    iInv "TINV" as "TI" "TI_CLOSE".
-    iEval (unfold tklockInv; simpl; red_tl_all) in "TI".
-    iDestruct "TI" as (o) "TI"; iEval (red_tl_all; simpl) in "TI".
-    iDestruct "TI" as (n) "TI"; iEval (red_tl_all; simpl) in "TI".
-    iDestruct "TI" as (κu) "TI"; iEval (red_tl_all; simpl) in "TI".
-    iDestruct "TI" as (D) "TI"; iEval (red_tl_all; simpl) in "TI".
-
-    destruct (Nat.eq_dec o n).
-    (* SUCCESS *) (* Required pcs : (1+l, 1) *)
-    { subst. iClear "CRED".
-      iDestruct "TI" as "(LOPT & LNPT & TB & SHOTS_BASE & %HD & HCOND & HWAIT)". rred2r.
-      (* FAA *)
-      iApply (SCMem_faa_fun_spec with "[LNPT MEM]"). auto.
+    iEval (rewrite unfold_iter_eq; rred2r).
+    iInv "INV" as "TI" "TI_CLOSE". iEval (simpl; unfold tklockInv; red_tl_all; simpl) in "TI".
+    iDestruct "TI" as (o2) "TI"; iEval (red_tl_all; simpl) in "TI".
+    iDestruct "TI" as (n2) "TI"; iEval (red_tl_all; simpl) in "TI".
+    iDestruct "TI" as (κu2) "TI"; iEval (red_tl_all; simpl) in "TI".
+    iDestruct "TI" as (γs2) "TI"; iEval (red_tl_all; simpl) in "TI".
+    iDestruct "TI" as (b2) "TI"; iEval (red_tl_all; simpl) in "TI".
+    iDestruct "TI" as (D2) "TI"; iEval (red_tl_all; simpl) in "TI".
+    iDestruct "TI" as "(LOPT & LNPT & TB & %HD & %HB & LB & HOWNER & HWAIT)".
+    iPoseProof (Ticket_black_issued with "TB ISSUED") as "%HIND2".
+    iDestruct "HOWNER" as "[(%EQ & _) | (#OBL2 & #PRM2 & #AO2 & PENDING2 & %κack2 & REST)]".
+    { subst; apply HD in HIND2; lia. }
+    assert (D2 = D2 ∖ {[n]} ∪ {[n]}).
+    { set_unfold. split; ii. destruct (Nat.eq_dec x n). subst. right; auto. left; auto.
+      des; subst; auto.
+    }
+    iEval (setoid_rewrite H; rewrite red_tl_big_sepS) in "HWAIT". rewrite big_opS_union; cycle 1. set_solver.
+    iDestruct "HWAIT" as "[HWAIT Hn]". rewrite big_sepS_singleton.
+    iEval (red_tl_all; simpl) in "Hn". iDestruct "Hn" as "[%EQ | (%HGT & %κu' & Hn)]".
+    { (* My turn *)
+      subst.
+      iEval (red_tl_all; simpl) in "REST". iDestruct "REST" as "(WAIT & [ISSUED' | LW])".
+      { iExFalso. iApply (Ticket_issued_twice with "ISSUED ISSUED'"). }
+      iPoseProof (Ticket_issued_wait with "ISSUED WAIT") as "%EQ". clarify.
+      iAssert (#=> ◇[κu2](1, 2))%I with "[PC]" as "> PC".
+      { destruct (Nat.eq_dec l 1). subst. done.
+        iMod (pc_drop _ 1 l _ 2 2 with "[PC]") as "PC". auto. done. done.
+      }
+      iMod ("TI_CLOSE" with "[- POST DUTY PC ISSUED PCS]") as "_".
+      { iEval (unfold tklockInv; simpl; red_tl_all).
+        iExists o2. iEval (red_tl; simpl). iExists n2. iEval (red_tl; simpl).
+        iExists κu2. iEval (red_tl; simpl). iExists γs2. iEval (red_tl; simpl).
+        iExists b2. iEval (red_tl; simpl). iExists D2. iEval (red_tl_all; simpl). iFrame.
+        iSplitR; auto. iSplitR; auto.
+        iSplitR "HWAIT".
+        { iRight. iFrame. repeat iSplitR; try done. iExists κack2. red_tl_all; simpl. iFrame. }
+        iEval (setoid_rewrite H; rewrite red_tl_big_sepS). rewrite big_opS_union; cycle 1. set_solver.
+        iSplitL; auto. iApply big_sepS_singleton. red_tl; iLeft; auto.
+      }
+      iApply (wpsim_yieldR2 with "[DUTY PCS PC]"). auto. instantiate (1:=2); auto.
+      { iSplitL "DUTY"; auto. iApply (pcs_cons_fold with "[PCS PC]"). iFrame. }
+      iIntros "DUTY _ PCS". simpl. rred2r.
+      clear n2 D2 HD HIND2 H HB. iClear "OBL2 PRM2".
+      iInv "INV" as "TI" "TI_CLOSE". iEval (simpl; unfold tklockInv; red_tl_all; simpl) in "TI".
+      iDestruct "TI" as (o3) "TI"; iEval (red_tl_all; simpl) in "TI".
+      iDestruct "TI" as (n3) "TI"; iEval (red_tl_all; simpl) in "TI".
+      iDestruct "TI" as (κu3) "TI"; iEval (red_tl_all; simpl) in "TI".
+      iDestruct "TI" as (γs3) "TI"; iEval (red_tl_all; simpl) in "TI".
+      iDestruct "TI" as (b3) "TI"; iEval (red_tl_all; simpl) in "TI".
+      iDestruct "TI" as (D3) "TI"; iEval (red_tl_all; simpl) in "TI".
+      iDestruct "TI" as "(LOPT & LNPT & TB & %HD & %HB & LB & HOWNER & HWAIT)".
+      iPoseProof (Ticket_black_issued with "TB ISSUED") as "%HIND3".
+      iDestruct "HOWNER" as "[(%EQ & _) | (#OBL & #PRM & _ & PENDING & %κack3 & REST)]".
+      { subst; apply HD in HIND3; lia. }
+      assert (D3 = D3 ∖ {[o2]} ∪ {[o2]}).
+      { set_unfold. split; ii. destruct (Nat.eq_dec x o2). subst. right; auto. left; auto.
+        des; subst; auto.
+      }
+      iEval (setoid_rewrite H; rewrite red_tl_big_sepS) in "HWAIT". rewrite big_opS_union; cycle 1. set_solver.
+      iDestruct "HWAIT" as "[HWAIT Ho2]". rewrite big_sepS_singleton.
+      iEval (red_tl_all; simpl) in "Ho2". iDestruct "Ho2" as "[%EQ | (%HGT & %κu2' & Ho2)]"; cycle 1.
+      { iEval (red_tl; simpl) in "Ho2". iDestruct "Ho2" as (κack2') "Ho2".
+        iEval (red_tl; simpl) in "Ho2". iDestruct "Ho2" as (γ2') "Ho2".
+        iEval (red_tl_all; simpl) in "Ho2". iDestruct "Ho2" as "(_ & _ & PO2 & _ & WAIT & _)".
+        iPoseProof (Ticket_issued_wait with "ISSUED WAIT") as "%EQ". clarify.
+        iExFalso. iApply (pending_not_active with "PO2 AO2").
+      }
+      subst. iApply (SCMem_load_fun_spec with "[LOPT] [-]"). auto.
       { pose proof mask_disjoint_ticketlock_state_tgt. set_solver. }
-      { iSplitR "LNPT"; done. }
-      iIntros (rv) "(%EQ & LNPT)". subst. iEval (ss) in "LNPT". rred2r. iApply wpsim_tauR. rred2r.
-      (* ALLOCATE TICKETS AND OBLIGATIONS TO PUT IN *)
-      iMod (alloc_obligation l 5) as "(%κu' & #OBL & PC & PO)". iEval (rewrite <- Qp.half_half) in "PO".
-      iPoseProof (pending_split _ (1/2) (1/2) with "PO") as "[PO PO']".
-      iPoseProof (pc_split _ _ 1 _ with "[PC]") as "[PC' PC]". simpl. done.
-      iAssert (#=> ◇[κu'](1, 1))%I with "[PC']" as "> PC'".
-      { destruct (Nat.eq_dec l 1); [subst; done | ].
-        iMod (pc_drop _ 1 l _ 1 1 with "[PC']") as "PC'". auto. done. done.
+      { iFrame. done. }
+      iIntros (rv) "[%EQ LOPT]". subst. rred2r. iApply wpsim_tauR. rred2r.
+      iEval (red_tl_all; simpl) in "REST". iDestruct "REST" as "(WAIT & [ISSUED' | [LW P]])".
+      { iExFalso. iApply (Ticket_issued_twice with "ISSUED ISSUED'"). }
+      iPoseProof (Ticket_issued_wait with "ISSUED WAIT") as "%EQ". clarify.
+      iMod (AuthExcls.b_w_update _ _ _ (κu3, γs3, b3) with "LB LW") as "(LB & LW)".
+      iMod ("TI_CLOSE" with "[- POST DUTY PCS LW P]") as "_".
+      { iEval (unfold tklockInv; simpl; red_tl_all).
+        iExists o3. iEval (red_tl; simpl). iExists n3. iEval (red_tl; simpl).
+        iExists κu3. iEval (red_tl; simpl). iExists γs3. iEval (red_tl; simpl).
+        iExists b3. iEval (red_tl; simpl). iExists D3. iEval (red_tl_all; simpl). iFrame.
+        iSplitR; auto. iSplitR; auto. iSplitR "HWAIT".
+        { iRight. iFrame. repeat iSplitR; try done. iExists κack3. red_tl_all; simpl. iFrame. }
+        iEval (setoid_rewrite H; rewrite red_tl_big_sepS). rewrite big_opS_union; cycle 1. set_solver.
+        iSplitL; auto. iApply big_sepS_singleton. red_tl; iLeft; auto.
       }
-      iPoseProof (duty_add with "[DUTY PC' PO'] []") as "> DUTY".
-      { iSplitL "DUTY"; [done | ]. iSplitL "PC'"; done. }
-      { instantiate (1:=(s_shots_shot γs n κu' : sProp i)%S). iModIntro. simpl.
-        red_tl_all. simpl. iIntros. iModIntro. done.
-      }
-      iPoseProof (duty_delayed_tpromise with "DUTY") as "#DPRM".
-      { simpl. left; auto. }
-      iMod (activate_tpromise with "DPRM PO") as "[#PRM #AO]". iClear "DPRM".
-      iMod (Ticket_alloc γt n D n κu' with "TB") as "(TB & ISSUED1 & WAIT)".
-      { intros H; apply HD in H; lia. }
-      iDestruct "HCOND" as "[TKL | [%κack' TCONT]]"; cycle 1.
-      { iEval (red_tl_all; simpl) in "TCONT". iDestruct "TCONT" as "(ISSUED2 & _)".
-        iExFalso. iApply (Ticket_issued_twice γt n with "[ISSUED1 ISSUED2]"). iFrame.
-      }
-      iDestruct "TKL" as "(TKL & P & [_ | [%NEQ _]])"; cycle 1. lia.
-      iMod (Shots_alloc κu' with "SHOTS_BASE") as "[SHOTS_BASE PENDING]".
-      (* CLOSE *)
-      iMod ("TI_CLOSE" with "[- POST PCS PCS' PC TKL P DUTY WAIT]") as "_".
-      { iEval (unfold tklockInv; simpl; red_tl_all). iExists n.
-        iEval (red_tl; simpl). iExists (n+1). iEval (red_tl; simpl). iExists κu'.
-        iEval (red_tl; simpl). iExists (D ∪ {[n]}). iEval (red_tl_all; simpl). iFrame.
-        iSplitL "SHOTS_BASE". { iEval (rewrite Nat.add_comm). done. }
-        iSplit.
-        { iPureIntro; auto. split; ii.
-          { destruct (Nat.eq_dec tk n); [set_solver|].
-            assert (HLT : tk < n) by lia; apply HD in HLT; set_solver.
-          }
-          { rewrite elem_of_union in H; destruct H.
-            { apply HD in H; lia. } { rewrite elem_of_singleton in H; clarify; lia. }
-          }
-        }
-        iSplitL "ISSUED1 PENDING".
-        { iRight. iExists κu'. red_tl_all. iFrame. simpl. iSplit; [done | iSplit; done]. }
-        { repeat rewrite red_tl_big_sepS. rewrite big_opS_union. iSplitL; cycle 1.
-          { rewrite big_sepS_singleton. red_tl_all. iRight; iLeft. done. }
-          { iApply (big_sepS_impl with "HWAIT"). iModIntro. iIntros "%x %HXD PRE".
-            red_tl_all. iLeft. iSplitR.
-            { iPureIntro. apply HD in HXD. lia. }
-            { iDestruct "PRE" as "[[%HLT H] | [%HEQ | [%HGT H]]]".
-              { done. }
-              { subst. apply HD in HXD; lia. }
-              { apply HD in HXD; lia. }
-            }
-          }
-          set_unfold. ii. subst. apply HD in H; lia.
-        }
-      }
-      clear κu. rename κu' into κu.
-      iEval (rewrite unfold_iter_eq; rred2r).
-      (* YIELD *)
-      iPoseProof (pc_split _ _ 3 _ with "PC") as "[PC' PC]".
-      iAssert (#=> ◇[κu](1, 3))%I with "[PC']" as "> PC'".
-      { destruct (Nat.eq_dec l 1); [subst; done | ].
-        iMod (pc_drop _ 1 l _ 3 3 with "[PC']") as "PC'". auto. done. done.
-      }
-      iApply (wpsim_yieldR2 with "[DUTY PCS' PC']").
-      { instantiate (1 := i). auto. }
-      { instantiate (1 := 3). auto. }
-      { iSplitL "DUTY". done.
-        iApply (pcs_cons_fold with "[PCS' PC']").
-        { iEval (rewrite Nat.add_comm). simpl. iSplitL "PC'"; done. }
-      }
-      iIntros "DUTY _ PCS'". simpl. rred2r.
-      (* LOAD - OPEN INVARIANT *)
-      iInv "TINV" as "TI" "TI_CLOSE".
-      iEval (unfold tklockInv; simpl; red_tl_all) in "TI".
-      iDestruct "TI" as (o') "TI"; iEval (red_tl_all; simpl) in "TI".
-      iDestruct "TI" as (n') "TI"; iEval (red_tl_all; simpl) in "TI".
-      iDestruct "TI" as (κu') "TI"; iEval (red_tl_all; simpl) in "TI".
-      iDestruct "TI" as (D') "TI"; iEval (red_tl_all; simpl) in "TI".
-      iDestruct "TI"
-        as "(LOPT & LNPT & TB & SHOTS_BASE & %HD' & [(TKL' & P' & _) | TISSUED] & HWAIT)".
-      { iExFalso; iApply (Ticket_locked_twice with "[TKL TKL']"). iSplitL "TKL"; done. }
-      iPoseProof (Ticket_black_locked with "[TKL TB]") as "%EQ".
-      iSplitL "TKL"; done. symmetry in EQ; subst.
-      (* LOAD *)
-      iApply (SCMem_load_fun_spec with "[LOPT]"). auto.
-      { pose proof mask_disjoint_ticketlock_state_tgt. set_solver. }
-      { iSplitR "LOPT"; done. }
-      iIntros (rv) "[%EQ LOPT]"; subst. rred2r. iApply (wpsim_tauR). rred2r.
-      (* CLOSE *)
-      iMod ("TI_CLOSE" with "[- POST PCS TKL P PC DUTY PCS' WAIT]") as "_".
-      { iEval (unfold tklockInv; simpl; red_tl_all). iExists n.
-        iEval (red_tl_all; simpl). iExists n'.
-        iEval (red_tl_all; simpl). iExists κu'.
-        iEval (red_tl_all; simpl). iExists D'.
-        iEval (red_tl_all; simpl).
-        iSplitL "LOPT"; auto. iSplitL "LNPT"; auto.
-        iSplitL "TB"; auto. iSplitL "SHOTS_BASE"; try done. iSplit. auto.
-        iSplitL "TISSUED". iRight. done. done.
-      }
-      clear n' HD' D' κu'.
-      (* YIELD *)
-      iCombine "DUTY" "PCS'" as "DUTY".
-      iApply (wpsim_yieldR2 with "DUTY"). auto. auto.
-      iIntros "DUTY _ PCS'".  rred2r.
-      (* COMPARE *)
+      iApply (wpsim_yieldR2 with "[DUTY PCS]"). auto. left.
+      { iSplitL "DUTY"; auto. }
+      iIntros "DUTY _ _". rred2r.
       iApply (SCMem_compare_fun_spec with "[MEM]"). auto.
       { pose proof mask_disjoint_ticketlock_state_tgt. set_solver. }
       { simpl. des_ifs. iApply (tgt_interp_as_equiv with "MEM"). iIntros. iSplit.
@@ -385,369 +279,293 @@ Section SPEC.
         { simpl. red_tl; simpl. iIntros "[? _]". done. }
       }
       iIntros (rv) "[%EQ _]". exploit EQ. auto. i; subst. rred2r. iApply wpsim_tauR. rred2r.
-      (* SYNC *)
-      iCombine "DUTY" "PCS'" as "DUTY".
-      iApply (wpsim_yieldR2 with "DUTY"). auto. auto.
-      iIntros "DUTY _ PCS'".  rred2r. simpl. iApply wpsim_tauR. rred2r.
-      (* POST *)
-      iEval (red_tl) in "POST".
-      iApply ("POST" with "[-]").
-      { iExists n. red_tl. iExists κu. simpl. red_tl. iExists κu. red_tl_all; simpl. iFrame. }
+      iApply ("POST" $! tt with "[DUTY LW P]"). iFrame.
     }
-    Unshelve. all: auto; try lia.
 
-    (* FAILURE *)
-    iDestruct "TI" as "(LOPT & LNPT & TB & SHOTS_BASE & %HD' & HCOND & HWAIT)". rred2r.
-    iApply (SCMem_faa_fun_spec with "[MEM LNPT]"). auto.
+    iEval (red_tl) in "Hn". iDestruct "Hn" as (κack') "Hn".
+    iEval (red_tl) in "Hn". iDestruct "Hn" as (γs') "Hn".
+    iEval (red_tl_all; simpl) in "Hn". iDestruct "Hn" as "(#OBL & #PRM & PO & PENDING & WAIT & PCa & #LINK)".
+    iPoseProof (Ticket_issued_wait with "ISSUED WAIT") as "%EQ". clarify.
+    iApply (wpsim_yieldR_gen_pending with "DUTY [PO] [PCS]"). auto.
+    instantiate (1:=ds). instantiate (1:=[(κu', 0, (▿ γs' ())%S)]). f_equal.
+    3:{ iApply (pps_cons_fold with "[PO]"). iSplitL; auto. iApply pps_nil. }
+    econs; auto. instantiate (1:=2). auto. done.
+    iIntros "DUTY CRED PPS PCS".
+    iMod (tpromise_progress with "[CRED]") as "[PCa' | #CONTRA]".
+    { iFrame. iApply "PRM2". }
+    2:{ iEval (simpl; red_tl_all) in "CONTRA".
+        iExFalso. iApply (OneShots.pending_not_shot with "PENDING2 CONTRA").
+    }
+    iMod (link_amplify with "[PCa']") as "PCa'". iFrame. done.
+    iMod ("IH" with "PCa'") as "IH".
+    iMod ("TI_CLOSE" with "[- IH POST PC ISSUED DUTY PCS]") as "_".
+    { iEval (unfold tklockInv; simpl; red_tl_all).
+      iExists o2. iEval (red_tl; simpl). iExists n2. iEval (red_tl; simpl).
+      iExists κu2. iEval (red_tl; simpl). iExists γs2. iEval (red_tl; simpl).
+      iExists b2. iEval (red_tl; simpl). iExists D2. iEval (red_tl_all; simpl). iFrame.
+      iSplitR; auto. iSplitR; auto. iSplitR "HWAIT PENDING WAIT PCa PPS".
+      { iRight. iFrame. repeat iSplitR; try done. iExists κack2. red_tl_all; simpl. iFrame. }
+      iEval (setoid_rewrite H; rewrite red_tl_big_sepS). rewrite big_opS_union; cycle 1. set_solver.
+      iSplitL "HWAIT"; auto. iApply big_sepS_singleton. red_tl; iRight; auto. iSplit; auto.
+      iExists κu'. red_tl. iExists κack'. red_tl. iExists γs'. red_tl_all; simpl; iFrame.
+      iPoseProof (pps_cons_unfold with "PPS") as "[PO _]". iFrame. repeat iSplit; auto.
+    }
+    iModIntro. rred2r.
+    iClear "OBL2 PRM2 AO2 LINK OBL PRM". clear o2 n2 D2 HD HIND2 H HGT κu2 κack2 γs2 b2 HB.
+    iInv "INV" as "TI" "TI_CLOSE". iEval (simpl; unfold tklockInv; red_tl_all; simpl) in "TI".
+    iDestruct "TI" as (o2) "TI"; iEval (red_tl_all; simpl) in "TI".
+    iDestruct "TI" as (n2) "TI"; iEval (red_tl_all; simpl) in "TI".
+    iDestruct "TI" as (κu2) "TI"; iEval (red_tl_all; simpl) in "TI".
+    iDestruct "TI" as (γs2) "TI"; iEval (red_tl_all; simpl) in "TI".
+    iDestruct "TI" as (b2) "TI"; iEval (red_tl_all; simpl) in "TI".
+    iDestruct "TI" as (D2) "TI"; iEval (red_tl_all; simpl) in "TI".
+    iDestruct "TI" as "(LOPT & LNPT & TB & %HD & %HB & LB & HOWNER & HWAIT)".
+    iApply (SCMem_load_fun_spec with "[LOPT] [-]"). auto.
+    { pose proof mask_disjoint_ticketlock_state_tgt. set_solver. }
+    { iFrame. done. }
+    iIntros (rv) "[%EQ LOPT]". subst. rred2r. iApply wpsim_tauR. rred2r.
+    iPoseProof (Ticket_black_issued with "TB ISSUED") as "%HIND2".
+    iDestruct "HOWNER" as "[(%EQ & _) | (#OBL2 & #PRM2 & #AO2 & PENDING2 & %κack2 & REST)]".
+    { subst; apply HD in HIND2; lia. }
+    assert (D2 = D2 ∖ {[n]} ∪ {[n]}).
+    { set_unfold. split; ii. destruct (Nat.eq_dec x n). subst. right; auto. left; auto.
+      des; subst; auto.
+    }
+    iEval (setoid_rewrite H; rewrite red_tl_big_sepS) in "HWAIT". rewrite big_opS_union; cycle 1. set_solver.
+    iDestruct "HWAIT" as "[HWAIT Ho2]". rewrite big_sepS_singleton.
+    iEval (red_tl_all; simpl) in "Ho2". iDestruct "Ho2" as "[%EQ | (%HGT & %κu & Ho2)]".
+    { (* My turn *)
+      subst.
+      iEval (red_tl_all; simpl) in "REST". iDestruct "REST" as "(WAIT & [ISSUED' | [LW P]])".
+      { iExFalso. iApply (Ticket_issued_twice with "ISSUED ISSUED'"). }
+      iPoseProof (Ticket_issued_wait with "ISSUED WAIT") as "%EQ". clarify.
+      iPoseProof (pc_split _ _ 1 with "PC") as "[PC _]".
+      iAssert (#=> ◇[κu2](1, 1))%I with "[PC]" as "> PC".
+      { destruct (Nat.eq_dec l 1). subst. done.
+        iMod (pc_drop _ 1 l _ 1 1 with "[PC]") as "PC". auto. done. done.
+      }
+      iMod ("TI_CLOSE" with "[- POST PC DUTY PCS LW P]") as "_".
+      { iEval (unfold tklockInv; simpl; red_tl_all).
+        iExists o2. iEval (red_tl; simpl). iExists n2. iEval (red_tl; simpl).
+        iExists κu2. iEval (red_tl; simpl). iExists γs2. iEval (red_tl; simpl).
+        iExists b2. iEval (red_tl; simpl). iExists D2. iEval (red_tl_all; simpl). iFrame.
+        iSplitR; auto. iSplitR; auto. iSplitR "HWAIT".
+        { iRight. iFrame. repeat iSplitR; try done. iExists κack2. red_tl_all; simpl. iFrame. }
+        iEval (setoid_rewrite H; rewrite red_tl_big_sepS). rewrite big_opS_union; cycle 1. set_solver.
+        iSplitL "HWAIT"; auto. iApply big_sepS_singleton. red_tl; iLeft; auto.
+      }
+      iApply (wpsim_yieldR2 with "[DUTY PC PCS]"). auto. left.
+      { iSplitL "DUTY"; auto. iApply (pcs_cons_fold with "[PCS PC]"). iFrame. }
+      iIntros "DUTY _ _". rred2r.
+      iApply (SCMem_compare_fun_spec with "[MEM]"). auto.
+      { pose proof mask_disjoint_ticketlock_state_tgt. set_solver. }
+      { simpl. des_ifs. iApply (tgt_interp_as_equiv with "MEM"). iIntros. iSplit.
+        { iIntros. simpl. red_tl; simpl. iSplit; [done | iPureIntro; auto]. }
+        { simpl. red_tl; simpl. iIntros "[? _]". done. }
+      }
+      iIntros (rv) "[%EQ _]". exploit EQ. auto. i; subst. rred2r. iApply wpsim_tauR. rred2r.
+      iApply ("POST" with "[DUTY LW P]"). iFrame.
+    }
+    {
+      iEval (red_tl) in "Ho2". iDestruct "Ho2" as (κack) "Ho2".
+      iEval (red_tl) in "Ho2". iDestruct "Ho2" as (γs) "Ho2".
+      iEval (red_tl_all; simpl) in "Ho2". iDestruct "Ho2" as "(#OBL & #PRM & PO & PENDING & WAIT & PCa & #LINK)".
+      iPoseProof (Ticket_issued_wait with "ISSUED WAIT") as "%EQ". clarify.
+      iApply (wpsim_yieldR_gen_pending with "DUTY [PO] [PCS]"). auto.
+      instantiate (1:=ds). instantiate (1:=[(κu, 0, (▿ γs ())%S)]). f_equal.
+      3:{ iApply (pps_cons_fold with "[PO]"). iSplitL; auto. iApply pps_nil. }
+      econs; auto. instantiate (1:=1). auto. done.
+      iIntros "DUTY _ PPS _".
+      iPoseProof (pps_cons_unfold with "PPS") as "[PO _]".
+      iMod ("TI_CLOSE" with "[- IH POST PC ISSUED DUTY]") as "_".
+      { iEval (unfold tklockInv; simpl; red_tl_all).
+        iExists o2. iEval (red_tl; simpl). iExists n2. iEval (red_tl; simpl).
+        iExists κu2. iEval (red_tl; simpl). iExists γs2. iEval (red_tl; simpl).
+        iExists b2. iEval (red_tl; simpl). iExists D2. iEval (red_tl_all; simpl). iFrame.
+        iSplitR; auto. iSplitR; auto. iSplitR "HWAIT PENDING WAIT PCa PO".
+        { iRight. iFrame. repeat iSplitR; try done. iExists κack2. iFrame. }
+        iEval (setoid_rewrite H; rewrite red_tl_big_sepS). rewrite big_opS_union; cycle 1. set_solver.
+        iSplitL "HWAIT"; auto. iApply big_sepS_singleton. red_tl; iRight; auto. iSplit; auto.
+        iExists κu. red_tl. iExists κack. red_tl. iExists γs. red_tl_all; simpl; iFrame. repeat iSplit; auto.
+      }
+      iModIntro. rred2r.
+      iApply (SCMem_compare_fun_spec); auto.
+      { simpl. des_ifs. lia. iApply (tgt_interp_as_equiv with "MEM"). iIntros. iSplit.
+        { iIntros. simpl. red_tl; simpl. iSplit; [done | iPureIntro; auto]. }
+        { simpl. red_tl; simpl. iIntros "[? _]". done. }
+      }
+      iIntros (rv) "[_ %NEQ]". exploit NEQ. ii. inv H0. lia. i; subst.
+      rred2r. iApply wpsim_tauR. rred2r. iApply wpsim_tauR.
+      iApply wpsim_stutter_mon. instantiate (1:=ps); auto. auto.
+      iApply ("IH" with "DUTY PC ISSUED POST").
+    }
+  Unshelve. all: auto; try lia.
+  Qed.
+
+  Lemma TicketLock_lock_spec
+        tid i
+        (E : coPset)
+        (IN : ⊤ ⊆ E)
+    :
+    ⊢ ∀ γt loc (P : sProp i) l b (ds : list (nat * nat * sProp i)),
+        [@ tid, i, E @]
+          ⧼⟦((syn_tgt_interp_as i sndl (fun m => (s_memory_black m))
+              ∗ (⤉ isTicketLock i γt loc P l b)
+              ∗ (⤉ (Duty(tid) ds))
+              ∗ ⤉ ◇{ds@1}(5 + l, 1))%S), 1+i⟧⧽
+            (OMod.close_itree Client (SCMem.mod gvs) (TicketLock.lock loc))
+            ⧼rv, ⟦(∃ (κu γs : τ{nat, 1+i}),
+                    (⤉ P)
+                    ∗ (⤉ ○ γt (κu, γs, b))
+                    ∗ (⤉ (Duty(tid) ((κu, 0, ▿ γs tt) :: ds)))
+                    ∗ ◇[κu](l, 1))%S, 1+i⟧⧽
+  .
+  Proof.
+    iIntros. iStartTriple. iIntros "PRE POST". unfold TicketLock.lock.
+    iApply wpsim_discard. apply IN.
+    unfold isTicketLock. iEval (red_tl_all; simpl; rewrite red_syn_tgt_interp_as) in "PRE".
+    iDestruct "PRE" as "(#MEM & PRE & DUTY & PCS)".
+    iDestruct "PRE" as (lo) "PRE". iEval (red_tl_all; simpl) in "PRE".
+    iDestruct "PRE" as (ln) "PRE". iEval (red_tl_all; simpl) in "PRE".
+    iDestruct "PRE" as (N) "PRE". iEval (red_tl_all; simpl; rewrite red_syn_inv) in "PRE".
+    iDestruct "PRE" as "(%SUB & %GT & %EQ & #TINV)". clarify.
+
+    (* YIELD *)
+    rred2r.
+    iMod (pcs_drop _ _ 1 _ _ 2 with "[PCS]") as "PCS". 2:{ iFrame. } auto.
+    iMod (pcs_decr _ _ 1 _ with "PCS") as "[PCS' PCS]". auto.
+    iMod (pcs_drop _ _ 1 _ 2 2 with "PCS'") as "PCS'". lia.
+    iMod (pcs_decr _ _ 1 _ with "PCS'") as "[PCS'' PCS']". auto.
+    iMod (pcs_drop _ _ 1 _ 1 2 with "PCS'") as "PCS'". lia.
+    iCombine "DUTY" "PCS'" as "DUTY".
+    iApply (wpsim_yieldR2 with "DUTY"). auto. lia.
+    iIntros "DUTY CRED PCS'". simpl.
+
+    (* OPEN *)
+    iInv "TINV" as "TI" "TI_CLOSE".
+    iEval (unfold tklockInv; simpl; red_tl_all) in "TI".
+    iDestruct "TI" as (o) "TI"; iEval (red_tl_all; simpl) in "TI".
+    iDestruct "TI" as (n) "TI"; iEval (red_tl_all; simpl) in "TI".
+    iDestruct "TI" as (κu) "TI"; iEval (red_tl_all; simpl) in "TI".
+    iDestruct "TI" as (γs) "TI"; iEval (red_tl_all; simpl) in "TI".
+    iDestruct "TI" as (pass) "TI"; iEval (red_tl_all; simpl) in "TI".
+    iDestruct "TI" as (D) "TI"; iEval (red_tl_all; simpl) in "TI".
+
+    subst. iClear "CRED".
+    iDestruct "TI" as "(LOPT & LNPT & TB & %HD & %HB & LB & HOWNER & HWAIT)". rred2r.
+    (* FAA *)
+    iApply (SCMem_faa_fun_spec with "[LNPT MEM]"). auto.
     { pose proof mask_disjoint_ticketlock_state_tgt. set_solver. }
     { iSplitR "LNPT"; done. }
-    iIntros (rv) "[%EQ LNPT]". subst. iEval (simpl) in "LNPT".
-    rred2r. iApply wpsim_tauR. rred2r.
-    iEval (rewrite unfold_iter_eq; simpl). rred2r.
-    iCombine "DUTY" "PCS'" as "DUTY".
-    iApply (wpsim_yieldR_gen2 with "DUTY"). auto. simpl. auto.
-    iIntros "DUTY _ PCS'". iEval (simpl) in "PCS'".
-    (* Add a delayed promise to the duty *)
-    iMod (alloc_obligation l 5) as "(%κu' & #OBLu' & PCu' & POu')".
-    iEval (rewrite <- Qp.half_half) in "POu'".
-    iPoseProof (pending_split _ (1/2) (1/2) with "POu'") as "[POu' POu'']".
-    iPoseProof (pc_split _ _ 1 _ with "[PCu']") as "[PCu'' PCu']". done. simpl.
-    iAssert (#=> ◇[κu'](1, 1))%I with "[PCu'']" as "> PCu''".
-    { destruct (Nat.eq_dec l 1). subst; auto. destruct (gt_dec l 1); try lia.
-      iMod (pc_drop _ 1 with "PCu''"); auto.
+    iIntros (rv) "(%EQ & LNPT)". subst. iEval (ss) in "LNPT". rred2r. iApply wpsim_tauR. rred2r.
+    (* Allocate delayed promise *)
+    iMod (OneShots.alloc) as "(%γs2 & PENDING2)".
+    iMod (alloc_obligation l 5) as "(%κu2 & #OBL2 & PC2 & PO2)". iEval (rewrite <- Qp.half_half) in "PO2".
+    iPoseProof (pending_split _ (1/2) (1/2) with "PO2") as "[PO2 PO2']".
+    iPoseProof (pc_split _ _ 1 _ with "[PC2]") as "[PC2' PC2]". simpl. done.
+    iAssert (#=> ◇[κu2](1, 1))%I with "[PC2']" as "> PC2'".
+    { destruct (Nat.eq_dec l 1); [subst; done | ].
+      iMod (pc_drop _ 1 l _ 1 1 with "[PC2']") as "PC2'". auto. done. done.
     }
-    iPoseProof (duty_add with "[DUTY PCu'' POu'] []") as "> DUTY".
-    { iSplitL "DUTY"; [done | ]. iSplitL "PCu''"; done. }
-    { instantiate (1:=(s_shots_shot γs n κu' : sProp i)%S). iModIntro. simpl.
+    iPoseProof (duty_add with "[DUTY PC2' PO2'] []") as "> DUTY".
+    { iSplitL "DUTY"; [done | ]. iSplitL "PC2'"; done. }
+    { instantiate (1:=(▿ γs2 tt)%S). iModIntro. simpl.
       red_tl_all. simpl. iIntros. iModIntro. done.
     }
-    iPoseProof (duty_delayed_tpromise with "DUTY") as "#DPRM".
+    iPoseProof (duty_delayed_tpromise with "DUTY") as "#DPRM2".
     { simpl. left; auto. }
-    (* Allocate obligation for acquiring the lock *)
-    iMod (alloc_obligation (1+l) (1 + (n - o))) as "(%κack' & #OBLack' & PCack' & POack')".
-    (* Allocate my ticket and shot ra *)
-    iMod (Ticket_alloc γt _ _ n κu' κack' with "TB") as "(TB & ISSUED & WAIT)".
-    { intros H; apply HD' in H; lia. }
-    iMod (Shots_alloc κu' with "SHOTS_BASE") as "(SHOTS_BASE & PENDING)".
-    (* Make a ccs to do inductive reasoning on *)
-    iMod (pcs_decr _ _ 1 _ with "PCS") as "[PCS'' PCS]". auto.
-    iMod (ccs_make with "[PCS'']") as "[CCS _]".
-    { iSplitR "PCS''". done. instantiate (1:=2). simpl. done. }
-    (* Extract a link and a promise from the lock holder *)
-    iAssert (⌜o < n⌝ ∗ ◆[κu, l] ∗ -[κu](0)-◇ ((s_shots_shot γs o κu : sProp i))%S)%I with "[TB HCOND]" as
-      "(%HGT & #OBLu & #PRMu)".
-    { iDestruct "HCOND" as
-        "[(TKL & P & [%EQ | (%NEQ & %obl_o & COND)]) | (%κack & HCOND)]".
-      { clarify. }
-      { iEval (red_tl_all; simpl) in "COND".
-        iDestruct "COND" as "(_ & #PRMU & _ & _ & #OBL_O)". iSplit; auto.
-      }
-      { red_tl. iDestruct "HCOND" as "(H & #PRMU & _ & _ & #OBL_O)". red_tl_all; simpl.
-        iPoseProof (Ticket_black_issued with "[H TB]") as "%H". iFrame.
-        enough (o ∈ D). apply HD' in H0. auto. set_solver.
-      }
-    }
-    iPoseProof (pc_split _ _ 1 _ with "[PCack']") as "[PCack'' PCack']". done.
-    iMod (link_new κu κack' l 0 0 with "[PCack'']") as "[#LINK1 _]".
-    { iFrame. done. }
-    (* CLOSING THE INVARIANT *)
-    iMod ("TI_CLOSE" with "[- POST PCS' PCu' DUTY POack' ISSUED PCS CCS]") as "_".
-    { iEval (unfold tklockInv; simpl; red_tl). iExists o.
-      iEval (red_tl; simpl). iExists (n + 1).
-      iEval (red_tl; simpl). iExists κu.
-      iEval (red_tl; simpl). iExists (D ∪ {[n]}).
-      iEval (red_tl_all; simpl). iFrame.
-      iSplitL "SHOTS_BASE". { iEval (rewrite Nat.add_comm). done. }
-      iSplit.
-      { iPureIntro. split; i.
-        { destruct (Nat.eq_dec tk n); [set_solver|].
-          assert (HLT : tk < n) by lia; apply HD' in HLT; set_solver.
+    iMod (alloc_obligation (1+l) (1 + pass + (b + 1) * (n - o))) as "(%κack2 & #OBLa2 & PCa2 & _)".
+    iPoseProof (pc_split _ _ 1 with "PCa2") as "[PCa2' PCa2]".
+    iMod (ccs_make κack2 (1+l) _ 2 _ with "[PCS]") as "[CCS _]".
+    { simpl. auto. }
+    iRename "PCS'" into "PCS".
+    iDestruct "HOWNER" as "[(%EQ & LW & P) | (#OBL & #PRM & #AO & PENDING & %κack & REST)]".
+    { subst.
+      iMod (Ticket_alloc _ D n [κu2; γs2; κack2; b] with "TB") as "(TB & ISSUED & WAIT)".
+      { ii. apply HD in H. lia. }
+      iMod (activate_tpromise with "DPRM2 PO2") as "[#PRM2 #AO2]". iClear "DPRM2".
+      iMod (link_new κu2 κack2 l 0 0 with "[PCa2']") as "[#LINK _]". auto.
+      iMod (AuthExcls.b_w_update _ _ _ (κu2, γs2, b) with "LB LW") as "(LB & LW)".
+      iMod ("TI_CLOSE" with "[- POST PCS PCS'' PC2 DUTY CCS ISSUED]") as "_".
+      { iEval (unfold tklockInv; simpl; red_tl_all).
+        iExists n. iEval (red_tl; simpl). iExists (n+1). iEval (red_tl; simpl).
+        iExists κu2. iEval (red_tl; simpl). iExists γs2. iEval (red_tl; simpl).
+        iExists b. iEval (red_tl; simpl). iExists (D ∪ {[n]}). iEval (red_tl_all; simpl). iFrame.
+        iSplit.
+        { iPureIntro; auto. split; ii.
+          { enough (tk = n). subst; set_solver. lia. }
+          { rewrite elem_of_union in H; destruct H.
+            { apply HD in H; lia. }
+            { rewrite elem_of_singleton in H; clarify; lia. }
+          }
         }
-        { rewrite elem_of_union in H; destruct H.
-          { apply HD' in H; lia. } { rewrite elem_of_singleton in H; clarify; lia. }
+        iSplit; auto.
+        iSplitR "HWAIT".
+        { iRight. iFrame. repeat iSplitR; try done. iExists κack2. iEval (red_tl_all). iFrame. iRight. iFrame. }
+        assert (D = ∅). apply elem_of_equiv_empty_L. ii. apply HD in H; lia. subst.
+        rewrite ! red_tl_big_sepS; simpl. rewrite big_opS_union. iSplitR.
+        { iApply big_sepS_empty. done. }
+        iApply (big_sepS_singleton); red_tl_all; iLeft. auto. set_solver.
+      }
+      iPoseProof (pc_split _ _ 2 with "PC2") as "[PC2' PC2]".
+      iApply (TicketLock_lock_loop_spec _ _ N with "[DUTY PCS'' PC2' CCS ISSUED]"). auto. apply GT.
+      { red_tl_all. iEval (rewrite red_syn_inv; rewrite red_syn_tgt_interp_as; simpl). iFrame. iSplit; done. }
+      red_tl_all; simpl. iIntros (_) "(DUTY & WL & P)". rred2r.
+      iPoseProof (pc_split _ _ 1 with "PC2") as "[PC2' PC2]".
+      iAssert (#=> ◇[κu2](1, 1))%I with "[PC2']" as "> PC2'".
+      { destruct (Nat.eq_dec l 1); [subst; done | ].
+        iMod (pc_drop _ 1 l _ 1 1 with "[PC2']") as "PC2'". auto. done. done.
+      }
+      iApply (wpsim_yieldR with "[DUTY PCS PC2']"). auto.
+      { iSplitL "DUTY". done. iApply (pcs_cons_fold with "[PCS PC2']"). iFrame. }
+      iIntros "DUTY _". rred2r. iApply wpsim_tauR. rred2r.
+      iApply ("POST" with "[-]"). iExists κu2. red_tl. iExists γs2. red_tl_all. iFrame.
+    }
+    {
+      iMod (link_new κu κack2 l 0 0 with "[PCa2']") as "[#LINK _]". auto.
+      iAssert (⌜o < n⌝)%I with "[REST TB]" as "%HON".
+      { iEval (red_tl_all) in "REST". iDestruct "REST" as "[WAIT _]".
+        iPoseProof (Ticket_black_wait with "TB WAIT") as "%H". iPureIntro. apply HD. auto.
+      }
+      iMod (Ticket_alloc _ D n [κu2; γs2; κack2; b] with "TB") as "(TB & ISSUED & WAIT)".
+      { ii. apply HD in H. lia. }
+      iMod ("TI_CLOSE" with "[- POST PCS PCS'' PC2 DUTY CCS ISSUED]") as "_".
+      { iEval (unfold tklockInv; simpl; red_tl_all).
+        iExists o. iEval (red_tl; simpl). iExists (n+1). iEval (red_tl; simpl).
+        iExists κu. iEval (red_tl; simpl). iExists γs. iEval (red_tl; simpl).
+        iExists pass. iEval (red_tl; simpl). iExists (D ∪ {[n]}). iEval (red_tl_all; simpl). iFrame.
+        iSplitR.
+        { iPureIntro; auto. split; ii.
+          { destruct (Nat.eq_dec tk n). subst; set_solver. rewrite elem_of_union. left. apply HD. lia. }
+          { rewrite elem_of_union in H; destruct H.
+            { apply HD in H; lia. }
+            { rewrite elem_of_singleton in H; clarify; lia. }
+          }
         }
+        iSplit; auto. 
+        iSplitR "HWAIT PENDING2 PO2 WAIT PCa2".
+        { iRight. iFrame. repeat iSplitR; try done. iExists κack. done. }
+        rewrite ! red_tl_big_sepS; simpl. rewrite big_opS_union. iSplitL "HWAIT"; auto.
+        iApply (big_sepS_singleton); red_tl_all; iRight. iSplit; auto.
+        iExists κu2. red_tl. iExists κack2. red_tl. iExists γs2. red_tl_all; simpl. iFrame.
+        repeat iSplit; auto.
+        ii. apply HD in H. apply elem_of_singleton in H0; subst. lia.
       }
-      iSplitL "HCOND".
-      { iDestruct "HCOND" as
-        "[(LOCKED_O & P & [ %EQ | (%NEQ & COND) ]) | HCOND]".
-        { lia. }
-        { iLeft. iFrame. iRight. iFrame. iPureIntro. lia. }
-        { iRight. iFrame. }
+      iPoseProof (pc_split _ _ 2 with "PC2") as "[PC2' PC2]".
+      iApply (TicketLock_lock_loop_spec _ _ N with "[DUTY PCS'' PC2' CCS ISSUED]"). auto. apply GT.
+      { red_tl_all. iEval (rewrite red_syn_inv; rewrite red_syn_tgt_interp_as; simpl). iFrame. iSplit; done. }
+      red_tl_all; simpl. iIntros (_) "(DUTY & WL & P)". rred2r.
+      iPoseProof (pc_split _ _ 1 with "PC2") as "[PC2' PC2]".
+      iAssert (#=> ◇[κu2](1, 1))%I with "[PC2']" as "> PC2'".
+      { destruct (Nat.eq_dec l 1); [subst; done | ].
+        iMod (pc_drop _ 1 l _ 1 1 with "[PC2']") as "PC2'". auto. done. done.
       }
-      { repeat rewrite red_tl_big_sepS. rewrite big_opS_union. iSplitL "HWAIT"; cycle 1.
-        { rewrite big_sepS_singleton. red_tl. iRight. iRight. iSplit.
-          { iPureIntro. lia. }
-          iExists κu'. red_tl_all; simpl. iExists κack'. red_tl_all; simpl. iFrame.
-          repeat iSplit; done.
-        }
-        done. set_unfold. ii. subst. apply HD' in H; lia.
-      }
+      iApply (wpsim_yieldR with "[DUTY PCS PC2']"). auto.
+      { iSplitL "DUTY". done. iApply (pcs_cons_fold with "[PCS PC2']"). iFrame. }
+      iIntros "DUTY _". rred2r. iApply wpsim_tauR. rred2r.
+      iApply ("POST" with "[-]"). iExists κu2. red_tl. iExists γs2. red_tl_all. iFrame.
     }
-    clear HD'. iClear "PRMu OBLu LINK1 POack' PCS' DPRM". clear κu D o n0 HGT.
-    iModIntro. rred2r.
-    (* Induction on CCS *)
-    iRevert "PCS DUTY POST ISSUED PCu'".
-    iMod (ccs_ind2 with "CCS [-]") as "IND".
-    2:{ iIntros "PCS". iMod (pcs_drop _ _ _ _ 2 1 with "PCS"). lia. iApply "IND". done. }
-    iModIntro. iExists 0. iIntros "IH". iModIntro. iIntros "PCS DUTY POST ISSUED PC".
-    (* Opening invariant *)
-    iInv "TINV" as "TI" "TI_CLOSE".
-    iEval (unfold tklockInv; simpl; red_tl) in "TI".
-    iDestruct "TI" as (o') "TI"; iEval (red_tl; simpl) in "TI".
-    iDestruct "TI" as (n') "TI"; iEval (red_tl; simpl) in "TI".
-    iDestruct "TI" as (κu) "TI"; iEval (red_tl; simpl) in "TI".
-    (* iDestruct "TI" as (γo') "TI"; iEval (red_tl; simpl) in "TI". *)
-    iDestruct "TI" as (D) "TI"; iEval (red_tl_all; simpl) in "TI".
-    iDestruct "TI" as "(LOPT & LNPT & TB & SHOTS_BASE & %HD' & TO & HWAIT)".
-    (* Load *)
-    iApply (SCMem_load_fun_spec with "[LOPT]"). auto.
-    { pose proof mask_disjoint_ticketlock_state_tgt; set_solver. }
-    { iSplit; iFrame. done. }
-    iIntros (rv) "[%EQ LOPT]". subst. rred2r. iApply wpsim_tauR. rred2r.
-    (* Yield *)
-    destruct (Nat.eq_dec o' n).
-    { (* Case 1 : My turn has arrived *)
-      subst. iDestruct "TO" as "[(LOCKED_N & P & [%HNN' | H]) | (%κu'' & WAIT)]".
-      { subst. iPoseProof (Ticket_black_issued with "[TB ISSUED]") as "%HIN". iFrame.
-        apply HD' in HIN. lia.
-      }
-      2:{ iEval (red_tl_all; simpl) in "WAIT".
-          iExFalso; iApply (Ticket_issued_twice with "[ISSUED WAIT]"). iDestruct "WAIT" as "[WAIT _]". iFrame.
-      }
-      iDestruct "H" as "(%HNN' & %κack & H)". iEval (red_tl_all; simpl) in "H".
-      iDestruct "H" as "(WAIT & #PRM & #AO & PENDING & _)".
-      iPoseProof (Ticket_issued_wait with "[ISSUED WAIT]") as "%EQ". iFrame. des; clarify.
-      iMod (pcs_drop _ _ _ _ 1 2 with "PCS") as "PCS". lia.
-      iPoseProof (pc_split _ _ 2 with "PC") as "[PC' PC]".
-      iAssert (#=> ◇[κu](1, 2))%I with "[PC]" as "> PC".
-      { destruct (Nat.eq_dec l 1). subst; auto. destruct (gt_dec l 1); try lia.
-        iMod (pc_drop _ 1 with "PC"); auto.
-      }
-      iApply (wpsim_yieldR_gen2 with "[PCS PC DUTY]"). instantiate (1:=i). auto. instantiate (1:=2); auto.
-      { iSplitL "DUTY". done. iApply (pcs_cons_fold); simpl. iSplitL "PC". iFrame. done. }
-      iIntros "DUTY _ PCS". simpl.
-      iMod ("TI_CLOSE" with "[- POST LOCKED_N P WAIT DUTY PCS PC']") as "_".
-      { iEval (unfold tklockInv; simpl; red_tl). iExists n.
-        iEval (red_tl; simpl). iExists n'. iEval (red_tl; simpl). iExists κu.
-        iEval (red_tl; simpl). iExists D. red_tl_all. iFrame.
-        iSplitR. auto. iRight. iExists κack. red_tl_all. simpl. iFrame.
-        iSplit; [done | iSplit; done].
-      }
-      iModIntro. rred2r.
-      iApply (SCMem_compare_fun_spec); auto.
-      { simpl. des_ifs. iApply (tgt_interp_as_equiv with "MEM"). iIntros. iSplit.
-        { iIntros. simpl. red_tl; simpl. iSplit; [done | iPureIntro; auto]. }
-        { simpl. red_tl; simpl. iIntros "[? _]". done. }
-      }
-      iIntros (rv) "[%EQ _]". exploit EQ. auto. i; subst. rred2r. iApply wpsim_tauR. rred2r.
-      iCombine "DUTY" "PCS" as "DUTY".
-      iApply (wpsim_yieldR2 with "DUTY"). auto. auto.
-      iIntros "DUTY _ PCS". rred2r. iApply (wpsim_tauR). rred2r.
-      iEval (red_tl) in "POST".
-      iApply ("POST" with "[-]").
-      { iExists n. red_tl. iExists κu. red_tl_all; iExists κack. red_tl_all; simpl. iFrame.
-        iPoseProof (pc_split _ l 1 1 with "PC'") as "[_ PC']". done. }
-    }
-    (* Case 2 : Not my turn yet *)
-    (* Get my duty out of invariant *)
-    iEval (rewrite red_tl_big_sepS) in "HWAIT".
-    iPoseProof (Ticket_black_issued with "[TB ISSUED]") as "%HNN'".
-    { iFrame. }
-    assert (D = ((D ∖ {[n]}) ∪ {[n]})).
-    { set_unfold. split; ii. destruct (Nat.eq_dec x n); auto. des; clarify; auto. }
-    iEval (setoid_rewrite H) in "HWAIT".
-    iEval (rewrite <- red_tl_big_sepS) in "HWAIT".
-    iEval (rewrite red_tl_big_sepS; red_tl; simpl) in "HWAIT".
-    rewrite big_opS_union; cycle 1. set_solver.
-    iDestruct "HWAIT" as "[H1 H2]".
-    rewrite big_sepS_singleton. iEval (red_tl_all; simpl) in "H2".
-    iDestruct "H2" as "[ (_ & % & ISSUED2) | H2 ]".
-    { iEval (red_tl_all; simpl) in "ISSUED2". iDestruct "ISSUED2" as "[% ISSUED2]".
-      iExFalso; iApply (Ticket_issued_twice with "[ISSUED ISSUED2]"). red_tl_all; simpl. iFrame.
-    }
-    iDestruct "H2" as "[%HNO | (%HNO & %κu'' & H2) ]".
-    { lia. }
-    iEval (red_tl; simpl) in "H2". iDestruct "H2" as (κack'') "H2".
-    iEval (red_tl_all; simpl) in "H2".
-    iDestruct "H2" as "(#DPRM & PO & WAIT & PENDING & PC' & #LINK & #OBL)".
-    iPoseProof (Ticket_issued_wait with "[ISSUED WAIT]") as "%EQ". iFrame. des; symmetry in EQ, EQ0; des; clarify.
-    iMod (pcs_drop _ _ _ _ 1 4 with "PCS") as "PCS". lia. Unshelve. all: auto.
-    iAssert (◆[κu, l] ∗ -[κu](0)-◇ (s_shots_shot γs o' κu)%S)%I with "[TO]" as "[#OBLu #PRMu']".
-    { iDestruct "TO" as "[(TKL & P & [%EQ | (%NEQ & %κack & COND)]) | (%κack & ISSUED)]".
-      { clarify. apply HD' in HNN'. lia. }
-      { iEval (red_tl_all; simpl) in "COND".
-        iDestruct "COND" as "(_ & ? & _ & _ & #?)". iSplit; done.
-      }
-      { red_tl_all. iDestruct "ISSUED" as "(_ & ? & _ & _ & ?)". iSplit; done. }
-    }
-    (* Yield *)
-    iApply (wpsim_yieldR_gen_pending with "DUTY [PO] [PCS]"). auto.
-    { instantiate (2:=[(κu', 0, s_shots_shot γs n κu')]). f_equal. }
-    3:{ iApply (pps_cons_fold with "[PO]"). iSplitL; auto. iApply pps_nil. }
-    { auto. } 2: done. auto.
-    iIntros "DUTY CRED PPS PCS".
-    iCombine "PRMu'" "CRED" as "C".
-    iMod (tpromise_progress with "C") as "PC_O".
-    iDestruct "PC_O" as "[PC_O | #DEAD]"; cycle 1.
-    { iEval (simpl; red_tl_all) in "DEAD".
-      iDestruct "TO" as "[(TKL & P & [%EQ | (%NEQ & %obl_o & COND)]) | (%tid' & ISSUED')]".
-      { clarify. apply HD' in HNN'. lia. }
-      { iEval (red_tl_all; simpl) in "COND".
-        iDestruct "COND" as "(_ & _ & _ & PENDINGu' & _)".
-        iExFalso. iApply (Shots_pending_not_shot with "[PENDINGu' DEAD]"). iFrame. done.
-      }
-      { iEval (red_tl_all; simpl) in "ISSUED'". iDestruct "ISSUED'" as "(_ & _ & _ & PENDING' & _)".
-        iExFalso; iApply (Shots_pending_not_shot with "[PENDING' DEAD]"). iFrame. done.
-      }
-    }
-    iMod (link_amplify with "[PC_O LINK]") as "PC_W". iFrame. done.
-    (* Close the invariant *)
-    iMod ("TI_CLOSE" with "[-IH POST ISSUED PC DUTY PCS PC_W]") as "_".
-    { iEval (unfold tklockInv; simpl; red_tl). iExists o'.
-      iEval (red_tl; simpl). iExists n'. iEval (red_tl; simpl). iExists κu.
-      iEval (red_tl; simpl). iExists D. red_tl_all; simpl. iFrame.
-      iSplitR. auto. iEval (rewrite H; rewrite red_tl_big_sepS).
-      rewrite big_opS_union; cycle 1. set_solver. iFrame.
-      rewrite big_sepS_singleton. red_tl. iRight. iRight. iSplit. auto.
-      iExists κu'. red_tl; simpl. iExists κack'. red_tl; simpl. red_tl_all; simpl. iFrame.
-      iSplitR; [done |]. iSplitL; [|iSplit; done].
-      iPoseProof (pps_cons_unfold with "PPS") as "[PO _]". done.
-    }
-    iModIntro. rred2r.
-    iApply (SCMem_compare_fun_spec); auto.
-    { simpl. des_ifs. iApply (tgt_interp_as_equiv with "MEM"). iIntros. iSplit.
-      { iIntros. simpl. red_tl; simpl. iSplit; [done | iPureIntro; auto]. }
-      { simpl. red_tl; simpl. iIntros "[? _]". done. }
-    }
-    iIntros (rv) "[_ %NEQ]". exploit NEQ. ii. inv H0. lia. i; subst.
-    rred2r. iApply wpsim_tauR. rred2r. iApply wpsim_tauR.
-    iEval (rewrite unfold_iter_eq). rred2r.
-
-    iInv "TINV" as "TI" "TI_CLOSE".
-    iEval (unfold tklockInv; simpl; red_tl) in "TI".
-    iDestruct "TI" as (o'') "TI"; iEval (red_tl; simpl) in "TI".
-    iDestruct "TI" as (n'') "TI"; iEval (red_tl; simpl) in "TI".
-    iDestruct "TI" as (κu'') "TI"; iEval (red_tl; simpl) in "TI".
-    iDestruct "TI" as (D'') "TI"; iEval (red_tl_all; simpl) in "TI". clear HD' HNN'.
-    iDestruct "TI" as "(LOPT & LNPT & TB & SHOTS_BASE & %HD' & TO & HWAIT)".
-    
-    destruct (Nat.eq_dec o'' n).
-    { (* My turn has arrived *)
-      subst. iDestruct "TO" as "[ (LOCKED_N & P & [ %HNN' | H ]) | [%tid' HISSUED]]".
-      { subst. iPoseProof (Ticket_black_issued with "[TB ISSUED]") as "%HIN". iFrame.
-        apply HD' in HIN. lia.
-      }
-      2:{ iEval (red_tl_all; simpl) in "HISSUED".
-          iDestruct "HISSUED" as "(ISSUED' & _)".
-          iExFalso; iApply (Ticket_issued_twice with "[ISSUED ISSUED']"). iFrame.
-      }
-      iDestruct "H" as "(%HNN' & %κack'' & H)". iEval (red_tl_all; simpl) in "H".
-      iDestruct "H" as "(WAIT & #PRMu'' & #AOu'' & PENDING & #OBLu'')".
-      iPoseProof (Ticket_issued_wait with "[WAIT ISSUED]") as "%EQ"; auto. iFrame. des; clarify.
-      iPoseProof (pc_split _ _ 1 with "PC") as "[PC' PC]".
-      iMod (pcs_decr _ _ 1 with "PCS") as "[PCS' PCS]". instantiate (1:=2). auto.
-      iAssert (#=> ◇[κu''](1, 1))%I with "[PC']" as "> PC'".
-      { destruct (Nat.eq_dec l 1). subst; auto. destruct (gt_dec l 1); try lia.
-        iMod (pc_drop _ 1 with "PC'"); auto.
-      }
-      iApply (wpsim_yieldR_gen with "[PCS' PC' DUTY]"). instantiate (1:=i). auto.
-      { iSplitL "DUTY". done. iApply (pcs_cons_fold); simpl. iSplitL "PC'". iFrame. done. }
-      iIntros "DUTY CRED2".
-      iMod ("TI_CLOSE" with "[LNPT TB SHOTS_BASE HWAIT PENDING LOPT ISSUED]") as "_".
-      { iEval (unfold tklockInv; simpl; red_tl). iExists n.
-        iEval (red_tl; simpl). iExists n''. iEval (red_tl; simpl). iExists κu''.
-        iEval (red_tl; simpl). iExists D''. red_tl_all; simpl. iFrame.
-        iSplitR. auto. iRight. iExists κack''. red_tl_all. iFrame. repeat iSplit; done.
-      }
-      iModIntro. rred2r.
-      iInv "TINV" as "TI" "TI_CLOSE".
-      iEval (unfold tklockInv; simpl; red_tl) in "TI".
-      iDestruct "TI" as (o''') "TI"; iEval (red_tl; simpl) in "TI".
-      iDestruct "TI" as (n''') "TI"; iEval (red_tl; simpl) in "TI".
-      iDestruct "TI" as (κu''') "TI"; iEval (red_tl; simpl) in "TI".
-      iDestruct "TI" as (D''') "TI"; iEval (red_tl_all; simpl) in "TI". clear HD' HNN'.
-      iDestruct "TI" as "(LOPT & LNPT & TB & TI)".
-      iPoseProof (Ticket_black_locked with "[LOCKED_N TB]") as "%EQ".
-      iSplitL "LOCKED_N"; done. symmetry in EQ; subst.
-      (* LOAD *)
-      iApply (SCMem_load_fun_spec with "[LOPT]"). auto.
-      { pose proof mask_disjoint_ticketlock_state_tgt. set_solver. }
-      { iSplitR "LOPT"; done. }
-      iIntros (rv) "[%EQ LOPT]"; subst. rred2r. iApply (wpsim_tauR). rred2r.
-      iPoseProof (pc_split _ _ 1 with "PC") as "[PC' PC]".
-      iAssert (#=> ◇[κu''](1, 1))%I with "[PC']" as "PC'".
-      { destruct (Nat.eq_dec l 1). subst; auto. destruct (gt_dec l 1); try lia.
-        iMod (pc_drop _ 1 with "PC'"); auto.
-      }
-      iMod "PC'". iMod (pcs_decr _ _ 1 with "PCS") as "[PCS' PCS]". auto.
-      iApply (wpsim_yieldR_gen with "[PCS' PC' DUTY]"). instantiate (1:=i). auto.
-      { iSplitL "DUTY". done. iApply (pcs_cons_fold); simpl. iSplitL "PC'". iFrame. done. }
-      iIntros "DUTY _".
-      iMod ("TI_CLOSE" with "[TB TI LNPT LOPT]") as "_".
-      { iEval (unfold tklockInv; simpl; red_tl). iExists n.
-        iEval (red_tl; simpl). iExists n'''. iEval (red_tl; simpl). iExists κu'''.
-        iEval (red_tl; simpl). iExists D'''. red_tl_all. iFrame.
-      }
-      iModIntro. rred2r.
-      iApply (SCMem_compare_fun_spec); auto.
-      { simpl. des_ifs. iApply (tgt_interp_as_equiv with "MEM"). iIntros. iSplit.
-        { iIntros. simpl. red_tl; simpl. iSplit; [done | iPureIntro; auto]. }
-        { simpl. red_tl; simpl. iIntros "[? _]". done. }
-      }
-      iIntros (rv) "[%EQ _]". exploit EQ. auto. i; subst. rred2r. iApply wpsim_tauR. rred2r.
-      iPoseProof (pc_split _ _ 1 with "PC") as "[PC' PC]".
-      iAssert (#=> ◇[κu''](1, 1))%I with "[PC']" as "PC'".
-      { destruct (Nat.eq_dec l 1). subst; auto. destruct (gt_dec l 1); try lia.
-        iMod (pc_drop _ 1 with "PC'"); auto.
-      }
-      iMod "PC'".
-      iApply (wpsim_yieldR with "[PCS PC' DUTY]"). instantiate (1:=i). auto.
-      { iSplitL "DUTY". done. iApply (pcs_cons_fold); simpl. iSplitL "PC'". iFrame. done. }
-      iIntros "DUTY _". rred2r. iApply (wpsim_tauR). rred2r.
-      iEval (red_tl) in "POST".
-      iApply ("POST" with "[-]").
-      { iExists n. red_tl. iExists κu''. red_tl. iExists κack''. red_tl_all; simpl. iFrame. }
-    }
-
-    iPoseProof (Ticket_black_issued with "[ISSUED TB]") as "%HNN'".
-    { iFrame. }
-    assert (D'' = ((D'' ∖ {[n]}) ∪ {[n]})).
-    { set_unfold. split; ii. destruct (Nat.eq_dec x n); auto. des; clarify; auto. }
-    iEval (setoid_rewrite H0; red_tl_all; simpl) in "HWAIT".
-    iEval (rewrite red_tl_big_sepS; red_tl; simpl) in "HWAIT".
-    rewrite big_opS_union; cycle 1. set_solver.
-    iDestruct "HWAIT" as "[H1 H2]".
-    rewrite big_sepS_singleton. iEval (red_tl_all; simpl) in "H2".
-    iDestruct "H2" as "[ (_ & TISSUED2) | H2 ]".
-    { iDestruct "TISSUED2" as (tid') "T". iEval (red_tl_all) in "T".
-      iDestruct "T" as (obl') "ISSUED2".
-      iExFalso; iApply (Ticket_issued_twice with "[ISSUED ISSUED2]"). red_tl_all. iFrame.
-    }
-    iDestruct "H2" as "[%HNO' | (%HNO' & %κu''' & H2) ]".
-    { lia. }
-    iEval (red_tl; simpl) in "H2". iDestruct "H2" as (obl_w'') "H2".
-    iEval (red_tl_all; simpl) in "H2".
-    iDestruct "H2" as "(#DPRMo' & PO & WAIT & PENDING & PCo' & #LINK1 & #OBLo')".
-    iPoseProof (Ticket_issued_wait with "[ISSUED WAIT]") as "%EQ". iFrame. des; clarify.
-    iApply (wpsim_yieldR_gen_pending with "DUTY [PO] [PCS]"). auto.
-    { instantiate (2:=[(κu''', 0, s_shots_shot γs n κu''')]). f_equal. }
-    3:{ iApply (pps_cons_fold with "[PO]"). iSplitL; auto. iApply pps_nil. }
-    { auto. } 2: done. lia.
-    iIntros "DUTY CRED PPS PCS".
-    iMod ("TI_CLOSE" with "[- POST IH ISSUED PC_W PC DUTY]") as "_".
-    { iEval (unfold tklockInv; simpl; red_tl). iExists o''.
-      iEval (red_tl; simpl). iExists n''. iEval (red_tl; simpl). iExists κu''.
-      iEval (red_tl; simpl). iExists D''. red_tl_all; simpl. iFrame.
-      iSplitR. auto. iEval (rewrite H0; rewrite red_tl_big_sepS).
-      rewrite big_opS_union; cycle 1. set_solver. iFrame.
-      rewrite big_sepS_singleton. red_tl. iRight. iRight. iSplit. auto.
-      iExists κu'''. red_tl; simpl. iExists obl_w''. red_tl; simpl.
-      red_tl_all; simpl. iFrame. repeat iSplit; auto.
-      iPoseProof (pps_cons_unfold with "PPS") as "[PO _]". done.
-    }
-    iModIntro. rred2r.
-    iMod ("IH" with "PC_W") as "IH". iApply ("IH" with "DUTY POST ISSUED PC").
-  Unshelve. all: auto.
+  Unshelve. all: auto; lia.
   Qed.
 
   Lemma TicketLock_unlock_spec
@@ -755,226 +573,209 @@ Section SPEC.
         (E : coPset)
         (IN : ⊤ ⊆ E)
     :
-    ⊢ ∀ γt γs lo ln (P : sProp i) l (ds : list (nat * nat * sProp i)) o κu κack,
+    ⊢ ∀ γt loc (P : sProp i) l b pass (ds : list (nat * nat * sProp i)) κu γs,
         [@ tid, i, E @]
           ⧼⟦((syn_tgt_interp_as i sndl (fun m => (s_memory_black m)))
-               ∗ (⤉ isTicketLock i γt γs (lo, ln) P l)
-               ∗ (⤉ P)
-               ∗ (⤉ s_ticket_locked γt o)
-               ∗ (⤉ Duty(tid) ((κu, 0, s_shots_shot γs o κu) :: ds))
-               ∗ ◇{((κu, 0, emp) :: ds)@1}(1, 3))%S, 1+i⟧⧽
-            (OMod.close_itree Client (SCMem.mod gvs) (TicketLock.unlock (lo, ln)))
-            ⧼rv, ⟦((⤉ Duty(tid) ds))%S, 1+i⟧⧽
+              ∗ (⤉ isTicketLock i γt loc P l b)
+              ∗ (⤉ P)
+              ∗ (⤉ ○ γt (κu, γs, pass))
+              ∗ (⤉ Duty(tid) ((κu, 0, ▿ γs tt) :: ds))
+              ∗ ◇{((κu, 0, emp) :: ds)@1}(1, 3))%S, 1+i⟧⧽
+            (OMod.close_itree Client (SCMem.mod gvs) (TicketLock.unlock loc))
+              ⧼rv, ⟦((⤉ Duty(tid) ds))%S, 1+i⟧⧽
   .
   Proof.
     (* PREPROCESS *)
     iIntros. iStartTriple.
-    iIntros "PRE POST". unfold TicketLock.unlock. rred2r.
+    iIntros "PRE POST". unfold TicketLock.unlock.
     iApply wpsim_discard. apply IN.
     iEval (red_tl_all; simpl; rewrite red_syn_tgt_interp_as; simpl; red_tl_all; simpl) in "PRE".
-    iDestruct "PRE" as "(#MEM & ISLOCK & P & LOCKED & WAIT & DUTY & PCS)".
+    iDestruct "PRE" as "(#MEM & ISLOCK & P & LW & DUTY & PCS)".
     iEval (unfold isTicketLock; red_tl_all; simpl) in "ISLOCK".
-    iDestruct "ISLOCK" as (lo') "ISLOCK". iEval (red_tl_all; simpl) in "ISLOCK".
-    iDestruct "ISLOCK" as (ln') "ISLOCK". iEval (red_tl_all; simpl) in "ISLOCK".
+    iDestruct "ISLOCK" as (lo) "ISLOCK". iEval (red_tl_all; simpl) in "ISLOCK".
+    iDestruct "ISLOCK" as (ln) "ISLOCK". iEval (red_tl_all; simpl) in "ISLOCK".
     iDestruct "ISLOCK" as (N) "ISLOCK". iEval (red_tl_all; simpl) in "ISLOCK".
-    iDestruct "ISLOCK" as "(%NAME & %HLGT & %HEQ & TINV)". symmetry in HEQ. inv HEQ.
-    iEval (rewrite red_syn_inv; simpl) in "TINV". iPoseProof "TINV" as "#TINV".
+    iDestruct "ISLOCK" as "(%NAME & %HLGT & %HEQ & INV)". clarify. rred2r.
+    iEval (rewrite red_syn_inv; simpl) in "INV". iPoseProof "INV" as "#INV".
     (* YIELD *)
     iApply (wpsim_yieldR2 with "[DUTY PCS]").
     instantiate (1:=i); auto. instantiate (1:=3); auto. iFrame. done.
-    iIntros "DUTY CRED PCS". rred2r.
+    iIntros "DUTY _ PCS". simpl. rred2r.
     (* OPEN INVARIANT *)
-    iInv "TINV" as "TI" "TI_CLOSE".
+    iInv "INV" as "TI" "TI_CLOSE".
     iEval (unfold tklockInv; simpl; red_tl_all; simpl) in "TI".
-    iDestruct "TI" as (o') "TI". iEval (red_tl; simpl) in "TI".
-    iDestruct "TI" as (n') "TI". iEval (red_tl; simpl) in "TI".
+    iDestruct "TI" as (o) "TI". iEval (red_tl; simpl) in "TI".
+    iDestruct "TI" as (n) "TI". iEval (red_tl; simpl) in "TI".
     iDestruct "TI" as (κu') "TI". iEval (red_tl; simpl) in "TI".
+    iDestruct "TI" as (γs') "TI". iEval (red_tl; simpl) in "TI".
+    iDestruct "TI" as (pass') "TI". iEval (red_tl; simpl) in "TI".
     iDestruct "TI" as (D) "TI". iEval (red_tl_all; simpl) in "TI".
-    iDestruct "TI" as "(LOPT & LNPT & TKB & SHOTS_BASE & %HD & [[LOCKED2 _] | [%κack' TI]] & HWAIT)".
-    { iExFalso; iApply (Ticket_locked_twice with "[LOCKED LOCKED2]"). iFrame. }
-    iPoseProof (Ticket_black_locked with "[TKB LOCKED]") as "%EQ". iFrame. symmetry in EQ; subst.
-    iEval (red_tl_all; simpl) in "TI". iDestruct "TI" as "(ISSUED & TI)".
-    iPoseProof (Ticket_issued_wait with "[ISSUED WAIT]") as "%EQ". iFrame. des; clarify.
+    iDestruct "TI" as
+      "(LOPT & LNPT & TB & %HD & %HB & LB &
+        [(_ & LW' & _) | (#OBL & #PRM & #AO & PENDING & %κack' & REST)] & HWAIT)".
+    { iExFalso. iApply (AuthExcls.w_w_false with "LW LW'"). }
+    iEval (red_tl_all; simpl) in "REST". iDestruct "REST" as "(WAIT & [ISSUED | [LW' _]])"; cycle 1.
+    { iExFalso. iApply (AuthExcls.w_w_false with "LW LW'"). }
+    iPoseProof (AuthExcls.b_w_eq with "LB LW") as "%EQ"; clarify. rename κack' into κack.
     (* LOAD *)
     iApply (SCMem_load_fun_spec with "[LOPT]"). instantiate (1:=i); auto.
     { pose proof mask_disjoint_ticketlock_state_tgt; set_solver. }
     { iFrame. done. }
     iIntros (rv) "[%EQ LOPT]". subst. rred2r. iApply wpsim_tauR. rred2r.
     (* CLOSE INVARIANT *)
-    iMod ("TI_CLOSE" with "[LNPT TKB SHOTS_BASE ISSUED TI HWAIT LOPT]") as "_".
-    { iEval (unfold tklockInv; simpl; red_tl; simpl). iExists o.
-      iEval (red_tl; simpl). iExists n'. iEval (red_tl; simpl). iExists κu.
-      iEval (red_tl; simpl). iExists D.
-      iEval (red_tl_all; simpl). iFrame. iSplit; auto. iRight. iExists κack. red_tl_all. iFrame.
+    iMod ("TI_CLOSE" with "[- POST DUTY PCS ISSUED]") as "_".
+    { iEval (unfold tklockInv; simpl; red_tl; simpl).
+      iExists o. iEval (red_tl; simpl). iExists n. iEval (red_tl; simpl).
+      iExists κu. iEval (red_tl; simpl). iExists γs. iEval (red_tl; simpl).
+      iExists pass. iEval (red_tl; simpl). iExists D. iEval (red_tl_all; simpl).
+      iFrame. iSplit; auto. iSplit; auto. iRight. iFrame. repeat iSplit; auto.
+      iExists κack. red_tl_all. iFrame. iRight; auto. iFrame.
     }
     (* YIELD *)
     iApply (wpsim_yieldR2 with "[DUTY PCS]").
-    instantiate (1:=i); auto. instantiate (1:=2); auto. iFrame.
-    iIntros "DUTY CRED2 PCS". rred2r. iEval (simpl) in "PCS".
+    instantiate (1:=i); auto. instantiate (1:=2); auto. iSplitL "DUTY"; iFrame.
+    iIntros "DUTY _ PCS". rred2r. simpl.
     (* OPEN INVARIANT *)
-    clear HD n' D.
-    iInv "TINV" as "TI" "TI_CLOSE".
-    iEval (unfold tklockInv; simpl; red_tl_all; simpl) in "TI".
-    iDestruct "TI" as (o') "TI". iEval (red_tl; simpl) in "TI".
-    iDestruct "TI" as (n) "TI". iEval (red_tl; simpl) in "TI".
-    iDestruct "TI" as (κu') "TI". iEval (red_tl; simpl) in "TI".
-    iDestruct "TI" as (D) "TI". iEval (red_tl_all; simpl) in "TI".
-    iDestruct "TI" as "(LOPT & LNPT & TKB & SHOTS_BASE & %HD & [[LOCKED2 _] | [%κack' TI]] & HWAIT)".
-    { iExFalso; iApply (Ticket_locked_twice with "[LOCKED LOCKED2]"). iFrame. }
-    iEval (red_tl_all; simpl) in "TI".
-    iDestruct "TI" as "(ISSUED & #PRM & #AO & PENDING & #OBL)".
-    iPoseProof (Ticket_black_locked with "[TKB LOCKED]") as "%EQ". iFrame. symmetry in EQ; subst.
-    iPoseProof (Ticket_issued_wait with "[ISSUED WAIT]") as "%EQ". iFrame. des; clarify.
-    iMod (Shots_pending_shot with "PENDING") as "#DEAD".
-    iMod (duty_fulfill (v:=i) with "[DUTY]") as "DUTY".
-    { simpl. iSplitL "DUTY". done. red_tl_all. iSplit; done. }
-    (* STORE *)
+    clear HD HB n D.
+    iInv "INV" as "TI" "TI_CLOSE". iEval (simpl; unfold tklockInv; red_tl_all; simpl) in "TI".
+    iDestruct "TI" as (o2) "TI"; iEval (red_tl_all; simpl) in "TI".
+    iDestruct "TI" as (n2) "TI"; iEval (red_tl_all; simpl) in "TI".
+    iDestruct "TI" as (κu2) "TI"; iEval (red_tl_all; simpl) in "TI".
+    iDestruct "TI" as (γs2) "TI"; iEval (red_tl_all; simpl) in "TI".
+    iDestruct "TI" as (pass2) "TI"; iEval (red_tl_all; simpl) in "TI".
+    iDestruct "TI" as (D2) "TI"; iEval (red_tl_all; simpl) in "TI".
+    iDestruct "TI" as "(LOPT & LNPT & TB & %HD & %HB & LB & HOWNER & HWAIT)".
+    iPoseProof (Ticket_black_issued with "TB ISSUED") as "%HIND2".
+    iDestruct "HOWNER" as "[(%EQ & _) | (#OBL2 & #PRM2 & #AO2 & PENDING2 & %κack2 & REST)]".
+    { subst; apply HD in HIND2; lia. }
+    assert (D2 = D2 ∖ {[o]} ∪ {[o]}).
+    { set_unfold. split; ii. destruct (Nat.eq_dec x o). subst. right; auto. left; auto.
+      des; subst; auto.
+    }
+    iEval (setoid_rewrite H; rewrite red_tl_big_sepS) in "HWAIT". rewrite big_opS_union; cycle 1. set_solver.
+    iDestruct "HWAIT" as "[HWAIT Ho]". rewrite big_sepS_singleton.
+    iEval (red_tl_all; simpl) in "Ho". iDestruct "Ho" as "[%EQ | (%HGT & %κu'' & Ho)]"; cycle 1.
+    { iEval (red_tl; simpl) in "Ho". iDestruct "Ho" as (κack'') "Ho".
+      iEval (red_tl; simpl) in "Ho". iDestruct "Ho" as (γs'') "Ho".
+      iEval (red_tl_all; simpl) in "Ho". iDestruct "Ho" as "(_ & _ & PO & _ & WAIT & _)".
+      iPoseProof (Ticket_issued_wait with "ISSUED WAIT") as "%EQ". clarify.
+      iExFalso. iApply (pending_not_active with "PO AO").
+    }
+    subst.
+    iEval (red_tl_all; simpl) in "REST". iDestruct "REST" as "(WAIT & [ISSUED' | [LW P]])".
+    { iExFalso. iApply (Ticket_issued_twice with "ISSUED ISSUED'"). }
+    iPoseProof (Ticket_issued_wait with "ISSUED WAIT") as "%EQ". clarify.
+    iClear "OBL PRM AO".
     iApply (SCMem_store_fun_spec with "[LOPT]"). instantiate (1:=i); auto.
     { pose proof mask_disjoint_ticketlock_state_tgt; set_solver. }
     { iFrame. done. }
     iIntros (rv) "LOPT". rred2r. iApply wpsim_tauR. rred2r.
-    (* ALLOCATE OBLIGATIONS *)
-    iMod (Ticket_update γt o (o + 1) with "[TKB LOCKED]") as "[TKB LOCKED]". iFrame.
+    (* Fulfill the unlocking duty *)
+    iMod (OneShots.pending_shot _ tt with "PENDING2") as "#DEAD2".
+    iMod (duty_fulfill with "[DUTY]") as "DUTY".
+    { iSplitL; auto. simpl; red_tl_all. iSplit; auto. }
+    iPoseProof (pcs_cons_unfold with "PCS") as "[_ PCS]".
+    iMod (Ticket_return with "TB ISSUED WAIT") as "TB".
     (* CLOSE INVARIANT *)
-    destruct (Nat.eq_dec n (o + 1)).
+    destruct (Nat.eq_dec n2 (o2 + 1)).
     (* CASE 1 : NO ONE WAITING *)
     { subst.
       iMod ("TI_CLOSE" with "[- POST PCS DUTY]") as "_".
-      { iEval (unfold tklockInv; simpl; red_tl; simpl). iExists (o + 1).
-        iEval (red_tl; simpl). iExists (o + 1). iEval (red_tl; simpl). iExists κu.
-        iEval (red_tl; simpl). iExists D. iEval (red_tl_all; simpl).
-        iFrame. iSplit; auto. iSplitL "LOCKED P".
-        { iLeft. iFrame. iLeft. auto. }
-        rewrite ! red_tl_big_sepS.
-        assert (D = D ∖ {[o]} ∪ {[o]}).
-        { assert (o ∈ D) by (apply HD; lia). set_unfold. split; ii.
-          destruct (Nat.eq_dec x o); [right | left]; auto. des; clarify; auto. }
-        rewrite H. rewrite ! big_opS_union; cycle 1. set_solver. set_solver.
-        iDestruct "HWAIT" as "[HWAIT HO]". iSplitL "HWAIT".
-        { iPoseProof (big_sepS_impl with "HWAIT") as "IMPL".
-          iApply "IMPL". iModIntro. iIntros (x) "%HIN HWAIT". red_tl_all.
-          iDestruct "HWAIT" as "[[%LT ISSUED] | HWAIT]".
-          { iLeft; iFrame. iPureIntro; lia. }
-          iDestruct "HWAIT" as "[%EQ | [%HGT HWAIT]]".
-          { subst. set_solver. }
-          enough (x < o). lia.
-          set_unfold in HIN. des. apply HD in HIN. lia.
-        }
-        rewrite ! big_sepS_singleton. red_tl_all. iLeft. iSplitR "ISSUED". iPureIntro; lia.
-        iExists κu. red_tl. iExists κack. red_tl_all. done.
+      { iEval (unfold tklockInv; simpl; red_tl; simpl).
+        iExists (o2 + 1). iEval (red_tl; simpl). iExists (o2 + 1). iEval (red_tl; simpl).
+        iExists κu2. iEval (red_tl; simpl). iExists γs2. iEval (red_tl; simpl).
+        iExists pass2. iEval (red_tl; simpl). iExists (D2 ∖ {[o2]}). iEval (red_tl_all; simpl).
+        iFrame. iSplit; auto.
+        { iPureIntro. split; ii. lia. set_unfold in H0. des. apply HD in H0. lia. }
+        iSplit; auto. iSplitL "LW P".
+        { iLeft. iFrame. auto. }
+        assert (D2 ∖ {[o2]} = ∅).
+        { apply elem_of_equiv_empty_L. ii. set_unfold in H0. des. apply HD in H0; lia. }
+        rewrite H0. rewrite red_tl_big_sepS. iApply big_sepS_empty. done.
       }
-      iPoseProof (pcs_cons_unfold with "PCS") as "[_ PCS]". simpl.
       iApply (wpsim_yieldR2 with "[DUTY PCS]").
       instantiate (1:=i); auto. instantiate (1:=1); auto. iFrame.
-      iIntros "DUTY CRED3 PCS". rred2r. iApply wpsim_tauR. rred2r.
-      iApply ("POST" with "[DUTY]"). simpl. red_tl; simpl. done.
+      iIntros "DUTY _ _". rred2r. iApply wpsim_tauR. rred2r.
+      iApply ("POST" with "[DUTY]"). red_tl; simpl. done.
     }
     (* CASE 2 : SOMEONE WAITING *)
-    iPoseProof (Ticket_black_issued with "[TKB ISSUED]") as "%HOIND". iFrame.
-    apply HD in HOIND.
-    assert (D = list_to_set (seq 0 o) ∪ {[o]} ∪ {[1+o]} ∪ list_to_set (seq (2 + o) (n - (2 + o)))).
-    { set_unfold. split; ii.
-      { apply HD in H. destruct (lt_dec x o).
-        { left. left. left. apply elem_of_list_In. apply in_seq. lia. }
-        { destruct (lt_dec x (1+o)).
-          { left. left. right. lia. }
-          destruct (lt_dec x (2+o)). left; right; auto. lia.
-          right. apply elem_of_list_In. apply in_seq. lia.
-        }
-      }
-      apply HD. destruct H.
-      { destruct H. destruct H. apply elem_of_list_In in H. apply in_seq in H. lia. lia. lia. }
-      apply elem_of_list_In in H. apply in_seq in H. lia.
+    assert (D2 ∖ {[o2]} = {[1+o2]} ∪ list_to_set (seq (2 + o2) (n2 - (2 + o2)))).
+    { set_unfold. split; ii. des.
+      { apply HD in H0. destruct (lt_dec x (2+o2)). left. lia. right. apply elem_of_list_In. apply in_seq. lia. }
+      des. subst. split; auto. apply HD in HIND2. apply HD. lia.
+      apply elem_of_list_In in H0. apply in_seq in H0. split. apply HD. all: lia.
     }
-    (* assert (D = ((D ∖ {[o + 1]}) ∪ {[o + 1]})). *)
-    (* { set_unfold. split; ii. destruct (Nat.eq_dec x (o + 1)); auto. des; clarify; auto. apply HD. lia. } *)
-    iEval (setoid_rewrite H) in "HWAIT".
-    iEval (rewrite red_tl_big_sepS; red_tl; simpl) in "HWAIT".
+    iEval (setoid_rewrite H0) in "HWAIT".
     rewrite ! big_opS_union; cycle 1.
-    { set_unfold. ii. apply elem_of_list_In in H0. apply in_seq in H0. lia. }
-    { set_unfold. ii. destruct H0. apply elem_of_list_In in H0. apply in_seq in H0. lia. lia. }
-    { set_unfold. ii. destruct H0. destruct H0. apply elem_of_list_In in H0, H1. apply in_seq in H0, H1. lia.
-      apply elem_of_list_In in H1; apply in_seq in H1; lia. 
-      clarify. apply elem_of_list_In in H1. apply in_seq in H1. lia. }
-    iDestruct "HWAIT" as "[[[HW1 HW2] HW3] HW4]".
-    iEval (rewrite big_sepS_singleton; red_tl_all; simpl) in "HW2".
-    iEval (rewrite big_sepS_singleton; red_tl_all; simpl) in "HW3".
-    iDestruct "HW2" as "[[%HW2 _]| [%HW2 | (%H' & % & HW2)]]"; [lia | | lia].
-    iDestruct "HW3" as "[[%HW3 _]| [%HW3 | (%H' & %κu' & HW3)]]"; [lia | lia | ].
-    iEval (red_tl; simpl) in "HW3". iDestruct "HW3" as (κack') "HW3".
-    iEval (red_tl_all; simpl) in "HW3".
-    iDestruct "HW3" as "(#DPRM' & PO' & WAIT' & PENDING' & PC' & #LINK' & #OBL')".
-    replace (S o - o) with 1 by lia.
-    iPoseProof (activate_tpromise with "DPRM' PO'") as "> [#PRM' #AO']".
+    { set_unfold. ii. apply elem_of_list_In in H2. apply in_seq in H2. lia. }
+    iDestruct "HWAIT" as "[HNEXT HWAIT]".
+    iEval (rewrite big_sepS_singleton; red_tl_all; simpl) in "HNEXT".
+    iDestruct "HNEXT" as "[%HNEXT | (_ & %κu3 & HNEXT)]"; [lia | ].
+    iEval (red_tl) in "HNEXT". iDestruct "HNEXT" as (κack3) "HNEXT".
+    iEval (red_tl) in "HNEXT". iDestruct "HNEXT" as (γs3) "HNEXT".
+    iEval (red_tl_all; simpl) in "HNEXT". iDestruct "HNEXT" as "(#OBL3 & #DPRM3 & PO3 & PENDING3 & WAIT3 & _)".
+    iPoseProof (activate_tpromise with "DPRM3 PO3") as "> [#PRM3 #AO3]". iClear "DPRM3". iClear "OBL2 PRM2 AO2".
+    iMod (AuthExcls.b_w_update _ _ _ (κu3, γs3, b) with "LB LW") as "[LB LW]".
     (* Make new links *)
-    iAssert ([∗ set] y ∈ (list_to_set (seq (2+o) (n - (2+o)))),
+    iAssert ([∗ set] y ∈ (list_to_set (seq (2+o2) (n2 - (2+o2)))),
               #=( ObligationRA.edges_sat )=>  
-                (⌜y > o + 1⌝
-                  ∗ (∃ κu κack,
-                    -[κu](0)-⧖ (s_shots_shot γs y)
-                    ∗ ⧖ [κu, (1/2)]
-                    ∗ Ticket_wait γt y κu κack
-                    ∗ Shots_pending γs y
-                    ∗ ◇[κack](S l, y - (o + 1))
-                    ∗ κu' -(0)-◇ κack
-                    ∗ ◆[κu, l])))%I with "[HW4]" as "HW4".
-    { iApply (big_sepS_impl with "[HW4]"); iFrame. iModIntro. iIntros (x) "%XIN H".
-      red_tl. iDestruct "H" as "[[%HLT HI] | [%HEQ | [%HGT HWAIT]]]".
+                (⌜y > o2 + 1⌝
+                  ∗ (∃ (κu4 κack4 γs4 : nat),
+                    (◆[κu4, l]) ∗ (-[κu4](0)-⧖ (▿ γs4 tt)%S) ∗ (⧖ [κu4, (1/2)]) ∗ (△ γs4 1)
+                    ∗ (Ticket_wait γt y [κu4; γs4; κack4; b])
+                    ∗ (◇[κack4](S l, b + (b + 1) * (y - (o2 + 1)))) ∗ (κu3 -(0)-◇ κack4))))%I
+      with "[HWAIT]" as "HWAIT".
+    { iApply (big_sepS_impl with "[HWAIT]"); iFrame. iModIntro. iIntros (x) "%XIN H".
+      red_tl. iDestruct "H" as "[%HEQ | [%HGT HWAIT]]".
       { set_unfold in XIN. apply elem_of_list_In in XIN. apply in_seq in XIN. lia. }
-      { subst. set_unfold in XIN. apply elem_of_list_In in XIN. apply in_seq in XIN. lia. }
-      iDestruct "HWAIT" as (κu'') "HWAIT". red_tl. iDestruct "HWAIT" as (κack'') "HWAIT". red_tl.
-      iDestruct "HWAIT" as "(#DPRM'' & PO'' & WAIT'' & PENDING'' & PC'' & #LINK'' & #OBL'')".
-      iPoseProof (pc_split _ _ 1 _ with "[PC'']") as "[PC''1 PC''2]".
-      { replace (x - o) with (1 + (x - (o + 1))) by lia. done. }
+      iDestruct "HWAIT" as (κu4) "HWAIT". red_tl. iDestruct "HWAIT" as (κack4) "HWAIT". red_tl.
+      iDestruct "HWAIT" as (γs4) "HWAIT". red_tl_all. simpl.
+      iDestruct "HWAIT" as "(#OBL4 & #DPRM4 & PO4 & PENDING4 & WAIT4 & PC4 & _)".
+      iPoseProof (pc_split _ _ 1 _ with "[PC4]") as "[PC4' PC4]".
+      { iPoseProof (pc_split _ _ pass2 with "PC4") as "[_ PC4]".
+        replace ((b + 1) * (x - o2)) with (1 + b + (b + 1) * (x - (o2 + 1))). done.
+        replace (x - (o2 + 1)) with (x - o2 - 1) by lia.
+        assert (H': x - o2 > 0). lia. revert H'. generalize (x - o2). induction n0; ii; try lia. }
       iSplitR.
       { iModIntro; iPureIntro. set_unfold in XIN; apply elem_of_list_In in XIN; apply in_seq in XIN. lia. }
-      { iPoseProof (link_new with "[PC''1]") as "[LINK _]".
-        iSplit. iApply "OBL'". instantiate (1:=0). done. iMod "LINK". iModIntro. red_tl_all; simpl.
-        iExists κu'', κack''. iFrame. iSplit; done.
+      { iPoseProof (link_new with "[PC4']") as "[LINK _]".
+        iSplit. iApply "OBL3". instantiate (1:=0). done. iMod "LINK". iModIntro.
+        iExists κu4, κack4, γs4. fold (Nat.add b ((b + 1) * (x - o2 - 1))). iFrame. repeat iSplit; done.
       }
     }
-    iMod (big_sepS_bupd with "HW4") as "HW4".
+    iMod (big_sepS_bupd with "HWAIT") as "HWAIT".
     iMod ("TI_CLOSE" with "[- POST PCS DUTY]") as "_".
-    { simpl. iEval (unfold tklockInv; simpl; red_tl; simpl). iExists (o + 1).
-      iEval (red_tl; simpl). iExists n. iEval (red_tl; simpl). iExists κu'.
-      iEval (red_tl; simpl). iExists D. iEval (red_tl_all; simpl).
-      iSplitL "LOPT"; auto. iSplitL "LNPT"; auto. iSplitL "TKB"; auto. iSplitL "SHOTS_BASE"; auto.
+    { simpl. iEval (unfold tklockInv; simpl; red_tl; simpl).
+      iExists (o2 + 1). iEval (red_tl; simpl). iExists n2. iEval (red_tl; simpl).
+      iExists κu3. iEval (red_tl; simpl). iExists γs3. iEval (red_tl; simpl).
+      iExists b. iEval (red_tl; simpl). iExists (D2 ∖ {[o2]}). iEval (red_tl_all; simpl). iFrame.
       iSplitR; auto.
-      iSplitR "ISSUED HW1 HW4".
-      { iLeft. iFrame. iRight. iSplit. iPureIntro; lia.
-        iExists κack'. red_tl_all; simpl. do 2 replace (o + 1) with (S o) by lia. iFrame.
-        repeat iSplit; done.
+      { iPureIntro. rewrite H0. split; ii.
+        { apply elem_of_union. destruct (Nat.eq_dec tk (1 + o2)). left; set_solver.
+          right. set_unfold. apply elem_of_list_In. apply in_seq. lia.
+        }
+        { apply HD in HIND2. apply elem_of_union in H1; des. apply elem_of_singleton in H1; subst; lia.
+          set_unfold in H1. apply elem_of_list_In in H1. apply in_seq in H1. lia.
+        }
+      }
+      iSplit; auto.
+      iSplitR "HWAIT".
+      { iRight. repeat iSplit; auto. iFrame.
+        iExists κack3. red_tl_all; simpl. do 2 replace (o2 + 1) with (S o2) by lia. iFrame. iRight. iFrame.
       }
       rewrite ! red_tl_big_sepS.
-      rewrite H. rewrite ! big_opS_union; cycle 1.
-      { set_unfold. ii. apply elem_of_list_In in H0. apply in_seq in H0. lia. }
-      { set_unfold. ii. destruct H0. apply elem_of_list_In in H0. apply in_seq in H0. lia. lia. }
-      { set_unfold. ii. destruct H0. destruct H0. apply elem_of_list_In in H0, H1. apply in_seq in H0, H1. lia.
-        apply elem_of_list_In in H1; apply in_seq in H1; lia. 
-        clarify. apply elem_of_list_In in H1. apply in_seq in H1. lia. }
-      iSplitR "HW4".
-      { iSplitL. iSplitL "HW1". iApply (big_sepS_impl with "HW1"). iModIntro. iIntros (x) "%XIN H".
-        red_tl. iDestruct "H" as "[[%HLT HI] | [%HEQ | [%HGT HWAIT]]]".
-        { iDestruct "HI" as (κux) "HI". red_tl.
-          iDestruct "HI" as (κackx) "HI". iLeft. iSplit; auto. iPureIntro; lia.
-          iExists κux. red_tl_all. iExists κackx; red_tl_all. done.
-        }
-        { subst. set_unfold in XIN. apply elem_of_list_In in XIN. apply in_seq in XIN. lia. }
-        { set_unfold in XIN. apply elem_of_list_In in XIN. apply in_seq in XIN. lia. }
-        { rewrite big_sepS_singleton. red_tl_all. iLeft. iSplit; auto. iPureIntro; lia.
-          iExists κu; red_tl; iExists κack; red_tl_all; done.
-        }
-        rewrite big_sepS_singleton. red_tl_all. iRight; iLeft; iPureIntro; lia.
-      }
-      iApply (big_sepS_impl with "HW4"). iModIntro. iIntros (x) "%XIN H".
-      iDestruct "H" as "(%HXO & %κux & %κackx & #DPRMx & POx & WAITx & PENDINGx & PCx & LINKx)".
-      red_tl_all. iRight; iRight. iSplit; [iPureIntro; auto | ].
-      iExists κux; red_tl; iExists κackx; red_tl_all; simpl; iFrame. done.
+      rewrite H0. rewrite ! big_opS_union; cycle 1.
+      { set_unfold. ii. apply elem_of_list_In in H2. apply in_seq in H2. lia. }
+      iSplitR "HWAIT".
+      { rewrite big_sepS_singleton. red_tl_all. iLeft; iPureIntro; lia. }
+      iApply (big_sepS_impl with "HWAIT"). iModIntro. iIntros (x) "%XIN H".
+      iDestruct "H" as "(%HXO & %κu4 & %κack4 & %γs4 & #OBL4 & #DPRM4 & PO4 & PENDING4 & WAIT4 & PC4 & #LINK4)".
+      red_tl_all. iRight. iSplit; auto.
+      iExists κu4; red_tl; iExists κack4; red_tl; iExists γs4; red_tl_all; simpl; iFrame. repeat iSplit; done.
     }
-    iPoseProof (pcs_cons_unfold with "PCS") as "[PC PCS]". simpl.
     iApply (wpsim_yieldR2 with "[DUTY PCS]").
     instantiate (1:=i); auto. instantiate (1:=1); auto. iFrame.
-    iIntros "DUTY CRED3 PCS". rred2r. iApply wpsim_tauR. rred2r.
+    iIntros "DUTY _ _". rred2r. iApply wpsim_tauR. rred2r.
     iApply ("POST" with "[DUTY]"). simpl. red_tl; simpl. done.
   Unshelve. all: auto.
   Qed.
