src/example/TicketLockRA.v
@@ -1,147 +1,129 @@
 From sflib Require Import sflib.
 From Fairness Require Import Any PCM IProp IPM IPropAux.
 From Fairness Require Import TemporalLogic.
-From Fairness Require Export AuthExclAnysRA.
+From Fairness Require Export AuthExclAnysRA AuthExclsRA.
 From stdpp Require Import gmap.
 
-
 Section Ticket.
+
   (* Resource for each ticket lock *)
-  Definition _TicketRA : URA.t :=
-    URA.prod (Auth.t (URA.prod (Excl.t nat) (GsetK.t (K:=nat)))) AuthExclAnysRA.
+  Definition _TicketRA : URA.t := (URA.prod (Auth.t (GsetK.t (K:=nat))) AuthExclAnysRA)%ra.
   Definition TicketRA : URA.t := (nat ==> _TicketRA)%ra.
 
   Context `{Σ : GRA.t}.
   Context {HasTicketRA : @GRA.inG TicketRA Σ}.
+  Context {AuthExclAnys : @GRA.inG (AuthExcls.t (nat * nat * nat))%ra Σ}.
 
   Definition TicketRA_Auth_base : _TicketRA :=
-    (((@Auth.black (URA.prod _ _) (Some 0 : Excl.t nat, Some ∅ : GsetK.t))
-        ⋅ (@Auth.white (URA.prod _ _) (Some 0 : Excl.t nat, Some ∅ : GsetK.t))),
-     ((fun k => (Auth.black (Some (tt ↑) : Excl.t Any.t) ⋅ Auth.white (Some (tt ↑) : Excl.t Any.t))) : AuthExclAnysRA)
-    ).
+    (((Auth.black (Some ∅ : GsetK.t)) ⋅ (Auth.white (Some ∅ : GsetK.t))),
+      (AuExAny_ra (fun k => gset_elem_of_dec k ∅))).
 
   Definition TicketRA_Auth : iProp :=
-    (∃ (U : nat), OwnM ((fun k => if (lt_dec k U)
-                        then ε
-                        else TicketRA_Auth_base) : TicketRA)).
+    (∃ (U : nat),
+      OwnM ((fun k => if (lt_dec k U) then ε else TicketRA_Auth_base) : TicketRA)
+        ∗ AuthExcls.rest (fun k => lt_dec k U) (0, 0, 0)).
 
-  Definition Ticket_black_ra (r : nat) (o : nat) (D : gset nat) : TicketRA :=
-    (maps_to_res r (((Auth.black (((Some o) : Excl.t nat, Some D : GsetK.t) : URA.prod _ _)),
-                      AuExAny_ra (fun k => gset_elem_of_dec k D)) : URA.prod _ _)).
-  Definition Ticket_black r o D := OwnM (Ticket_black_ra r o D).
-
-  Definition Ticket_locked_ra (r o : nat) : TicketRA :=
-    (maps_to_res r ((Auth.white (((Some o) : Excl.t nat, Some ∅ : GsetK.t) : URA.prod _ _), ε) : URA.prod _ _)).
-  Definition Ticket_locked r o := OwnM (Ticket_locked_ra r o).
+  Definition Ticket_black_ra (γt : nat) (D : gset nat) : TicketRA :=
+    (maps_to_res γt (((Auth.black (Some D : GsetK.t)),
+                      (AuExAny_ra (fun k => gset_elem_of_dec k D))) : _TicketRA))%ra.
+  Definition Ticket_black γt D := OwnM (Ticket_black_ra γt D).
 
   (* The issuing thread holds my ticket -> (my thread id, and my obligation id). *)
-  Definition Ticket_issued_ra (r : nat) (m κu κack : nat) : TicketRA :=
-    (maps_to_res r ((Auth.white ((ε : Excl.t nat, Some {[m]} : GsetK.t) : URA.prod _ _),
-                     AuExAnyW_ra m (κu, κack)) : URA.prod _ _)).
-  Definition Ticket_issued r m κu κack := OwnM (Ticket_issued_ra r m κu κack).
+  Definition Ticket_issued_ra (γt : nat) (tk : nat) (l : list nat) : TicketRA :=
+    (maps_to_res γt (((Auth.white (Some {[tk]} : GsetK.t)), AuExAnyW_ra tk l) : _TicketRA)).
+  Definition Ticket_issued γt tk l := OwnM (Ticket_issued_ra γt tk l).
 
   (* The invariant holds ticket -> (thread id, obligation id) for the waiting threads. *)
-  Definition Ticket_wait_ra (r : nat) (m κu κack : nat) : TicketRA :=
-    (maps_to_res r ((Auth.white ((ε : Excl.t nat, Some ∅ : GsetK.t) : URA.prod _ _),
-                     AuExAnyB_ra m (κu, κack)) : URA.prod _ _)).
-  Definition Ticket_wait r m κu κack := OwnM (Ticket_wait_ra r m κu κack).
+  Definition Ticket_wait_ra (γt : nat) (tk : nat) (l : list nat) : TicketRA :=
+    (maps_to_res γt ((Auth.white (Some ∅ : GsetK.t), AuExAnyB_ra tk l) : _TicketRA)).
+  Definition Ticket_wait γt tk l := OwnM (Ticket_wait_ra γt tk l).
 
   (** Properties. *)
-  Lemma Ticket_locked_twice (r m1 m2: nat) : Ticket_locked r m1 ∗ Ticket_locked r m2 ⊢ False.
+  Lemma Ticket_issued_twice (γt tk : nat) (l l' : list nat) :
+    Ticket_issued γt tk l -∗ Ticket_issued γt tk l' -∗ False.
   Proof.
-    iStartProof. iIntros "[T1 T2]". unfold Ticket_locked, Ticket_locked_ra.
+    iStartProof. iIntros "T1 T2". unfold Ticket_issued, Ticket_issued_ra.
     iCombine "T1" "T2" as "T3".  iPoseProof (OwnM_valid with "T3") as "%T".
     setoid_rewrite maps_to_res_add in T. ur in T.
-    specialize (T r). ur in T. unfold maps_to_res in T. des_ifs. des.
-    ur in T. ur in T. des. ur in T. clarify.
+    specialize (T γt). ur in T. unfold maps_to_res in T. des_ifs. des.
+    repeat ur in T. des_ifs. set_solver.
   Qed.
 
-  Lemma Ticket_issued_twice (r m κu κack κu' κack' : nat) :
-    Ticket_issued r m κu κack ∗ Ticket_issued r m κu' κack' ⊢ False.
+  Lemma Ticket_black_issued (γt tk : nat) l D :
+    Ticket_black γt D -∗ Ticket_issued γt tk l -∗ ⌜tk ∈ D⌝.
   Proof.
-    iStartProof. iIntros "[T1 T2]". unfold Ticket_issued, Ticket_issued_ra.
-    iCombine "T1" "T2" as "T3".  iPoseProof (OwnM_valid with "T3") as "%T".
-    setoid_rewrite maps_to_res_add in T. ur in T.
-    specialize (T r). ur in T. unfold maps_to_res in T. des_ifs. des.
-    repeat ur in T. des_ifs. set_solver. des. auto.
-  Qed.
-
-  Lemma Ticket_black_locked (r m1 m2: nat) D : Ticket_locked r m1 ∗ Ticket_black r m2 D ⊢ ⌜m1 = m2⌝.
-  Proof.
-    iStartProof. iIntros "[T1 T2]". unfold Ticket_locked, Ticket_locked_ra, Ticket_black, Ticket_black_ra.
-    iCombine "T1" "T2" as "T3".  iPoseProof (OwnM_valid with "T3") as "%T".
-    setoid_rewrite maps_to_res_add in T. ur in T.
-    specialize (T r). ur in T. unfold maps_to_res in T. des_ifs. des.
-    ur in T. des_ifs. des.
-    destruct T. ur in H. des_ifs. ur in H1. des_ifs.
-    set_solver.
-  Qed.
-
-  Lemma Ticket_black_issued (r m1 m2 κu κack : nat) D :
-    Ticket_black r m1 D ∗ Ticket_issued r m2 κu κack ⊢ ⌜m2 ∈ D⌝.
-  Proof.
-    iStartProof. iIntros "[BLACK ISSUED]". unfold Ticket_black, Ticket_issued.
+    iStartProof. iIntros "BLACK ISSUED". unfold Ticket_black, Ticket_issued.
     iCombine "BLACK" "ISSUED" as "H". unfold Ticket_black_ra, Ticket_issued_ra.
     iPoseProof (OwnM_valid with "H") as "%H". setoid_rewrite maps_to_res_add in H.
-    ur in H. specialize (H r). unfold maps_to_res in H. des_ifs.
-    ur in H. des. ur in H. des. destruct H. des_ifs.
-    ur in H. des_ifs. destruct c0; ss. des_ifs; ss. 2:{ ur in H. ss. }
-    destruct c2; ss. 2:{ ur in H. ss. } ur in H. des_ifs. iPureIntro. set_solver.
+    ur in H. specialize (H γt). unfold maps_to_res in H. des_ifs.
+    ur in H. des. rewrite URA.unit_idl in H. ur in H. des. destruct H.
+    ur in H. des_ifs. iPureIntro; set_solver.
   Qed.
 
-  Lemma TicketRA_alloc o :
-    TicketRA_Auth ⊢ ∃ r, |==> TicketRA_Auth ∗ Ticket_black r o ∅ ∗ Ticket_locked r o.
+  Lemma Ticket_black_wait (γt tk : nat) l D :
+    Ticket_black γt D -∗ Ticket_wait γt tk l -∗ ⌜tk ∈ D⌝.
   Proof.
-    iIntros "[%U BASE]". iExists U.
+    iStartProof. iIntros "BLACK WAIT". unfold Ticket_black, Ticket_wait.
+    iCombine "BLACK" "WAIT" as "H". unfold Ticket_black_ra, Ticket_wait_ra, AuExAnyB_ra, AuExAny_ra.
+    iPoseProof (OwnM_valid with "H") as "%H". setoid_rewrite maps_to_res_add in H.
+    ur in H. specialize (H γt). unfold maps_to_res in H. des_ifs.
+    ur in H. des. des_ifs. ur in H0. specialize (H0 tk). des_ifs. ur in H0. auto.
+  Qed.
+
+  Lemma TicketRA_alloc κu γs b :
+    TicketRA_Auth ⊢ ∃ γt, |==> TicketRA_Auth ∗ Ticket_black γt ∅ ∗ ● γt (κu, γs, b) ∗ ○ γt (κu, γs, b).
+  Proof.
+    iIntros "[%U [BASE BASE2]]". iExists U.
     assert (URA.updatable
-      ((λ k, if lt_dec k U then ε else TicketRA_Auth_base) : TicketRA)
+      (((λ k, if lt_dec k U then ε else TicketRA_Auth_base) : TicketRA))
       (((λ k, if lt_dec k (S U) then ε else TicketRA_Auth_base) : TicketRA)
         ⋅ (maps_to_res U TicketRA_Auth_base))) as UPD.
     { ur. apply pointwise_updatable. i. unfold maps_to_res. des_ifs; try lia.
       - rewrite URA.unit_idl. reflexivity.
       - rewrite URA.unit_idl. reflexivity.
-      - rewrite URA.unit_id. reflexivity.  }
+      - rewrite URA.unit_id. reflexivity.
+    }
     iMod (OwnM_Upd with "BASE") as "[A B]". apply UPD.
-    assert (URA.updatable
-      (maps_to_res U TicketRA_Auth_base)
-      (Ticket_black_ra U o ∅
-        ⋅ maps_to_res U ((Auth.white ((Some o : Excl.t nat, Some ∅ : GsetK.t) : URA.prod _ _), ε) : URA.prod _ _))).
-    { ur. apply pointwise_updatable. i.
-      unfold Ticket_black_ra, Ticket_locked_ra, maps_to_res, TicketRA_Auth_base.
-      des_ifs; cycle 1. rewrite URA.unit_id. reflexivity.
-      rewrite ! URA.unfold_add. do 2 rewrite <- URA.unfold_add. ss. apply URA.prod_updatable.
-      { apply Auth.auth_update. ii. des. ur in FRAME. des_ifs. ur in H0. ur in H1. des_ifs. split.
-        ur. split; ur; auto. ur. f_equal. ur; auto. ur. des_ifs. rewrite <- H0; auto. }
-      unfold AuExAny_ra.
-      apply pointwise_updatable. ii. ss. ur in H. des_ifs. des.
-      rewrite URA.unit_idl in H. destruct H. ur in H.  des_ifs. rewrite URA.unit_id. ur. des_ifs.
-      split. exists ε. ur. des_ifs. ur. auto. }
-    iMod (OwnM_Upd with "B") as "[C D]". apply H.
-    iModIntro. iSplitL "A".
-    { iExists (S U). auto. }
-    { iSplitL "C". auto. unfold Ticket_locked, Ticket_locked_ra. auto. }
+    assert (URA.updatable (maps_to_res U TicketRA_Auth_base) (Ticket_black_ra U ∅)).
+    { unfold TicketRA_Auth_base, Ticket_black_ra.
+      apply maps_to_updatable. apply URA.prod_updatable; [ | reflexivity].
+      apply Auth.auth_dealloc. ii. des. ur in FRAME. des_ifs. split; ss.
+      rewrite URA.unit_idl. f_equal. set_solver.
+    }
+    iMod (OwnM_Upd with "B") as "D". apply H.
+    assert (URA.updatable (maps_to_res U TicketRA_Auth_base) (Ticket_black_ra U ∅)).
+    { unfold TicketRA_Auth_base, Ticket_black_ra.
+      apply maps_to_updatable. apply URA.prod_updatable; [ | reflexivity].
+      apply Auth.auth_dealloc. ii. des. ur in FRAME. des_ifs. split; ss.
+      rewrite URA.unit_idl. f_equal. set_solver.
+    }
+    iMod (AuthExcls.alloc_gen (gt_dec U) (gt_dec (S U)) with "BASE2") as "(BASE2 & B)".
+    { ii; des_ifs. lia. }
+    iAssert (#=> OwnM (AuthExcls.black_ra U (κu, γs, b) ⋅ AuthExcls.white_ra U (κu, γs, b)))%I with "[B]" as "> B".
+    { unfold AuthExcls.black_ra, AuthExcls.white_ra. setoid_rewrite maps_to_res_add.
+      iApply (OwnM_Upd with "B"). unfold maps_to_res. apply pointwise_updatable. i.
+      des_ifs; try lia. apply Auth.auth_update. ii. des. ur in FRAME. des_ifs. ur; split; auto. }
+    iModIntro; iFrame. iSplitR "B".
+    { iExists (S U). iFrame. }
+    iDestruct "B" as "[B B']". iSplitL "B"; done.
   Qed.
 
-  Lemma Ticket_alloc r o D new κu κack
+  Lemma Ticket_alloc γt D new l
     (NOTIN : new ∉ D)
     :
-    Ticket_black r o D ⊢
-      |==> Ticket_black r o (D ∪ {[new]}) ∗ Ticket_issued r new κu κack ∗ Ticket_wait r new κu κack.
+    Ticket_black γt D ⊢ |==> Ticket_black γt (D ∪ {[new]}) ∗ Ticket_issued γt new l ∗ Ticket_wait γt new l.
   Proof.
-    iIntros "TB". unfold Ticket_black, Ticket_issued.
-    assert (URA.updatable (Ticket_black_ra r o D)
-      (Ticket_black_ra r o (D ∪ {[new]}) ⋅ Ticket_issued_ra r new κu κack ⋅ Ticket_wait_ra r new κu κack)).
+    iIntros "TB". unfold Ticket_black, Ticket_issued, Ticket_wait.
+    assert (URA.updatable (Ticket_black_ra γt D)
+      (Ticket_black_ra γt (D ∪ {[new]}) ⋅ Ticket_issued_ra γt new l ⋅ Ticket_wait_ra γt new l)).
     { unfold Ticket_black_ra, Ticket_issued_ra, Ticket_wait_ra. do 2 setoid_rewrite maps_to_res_add.
       apply maps_to_updatable. ur. apply URA.prod_updatable.
-      { etrans.
-        { apply Auth.auth_alloc2. instantiate (1:= (ε, Some ({[new]}))). ur.
-          split; ur; des_ifs. set_solver. }
-        { setoid_rewrite <- URA.add_assoc. ur.
-          rewrite ! URA.unit_id. rewrite ! URA.unit_idl. ur. des_ifs; cycle 1. set_solver.
-          rewrite ! URA.unit_id. rewrite URA.unfold_add. ss. des_ifs; cycle 1. set_solver.
-          ii. ur in H. des_ifs. des. ur. split; cycle 1. ur. split; ur; auto.
-          destruct H. exists x. ur. des_ifs. ur in H. inv H. rewrite H2. rewrite H3. f_equal.
-          rewrite <- H3. enough (({[new]} ∪ ∅ : gset nat) = {[new]}). rewrite H; auto. set_solver. }
+      etrans.
+      { apply Auth.auth_alloc2. instantiate (1:= (Some ({[new]}))). ur.
+        ur; des_ifs. set_solver. }
+      { setoid_rewrite <- URA.add_assoc. ur.
+        rewrite ! URA.unit_idl. ur. des_ifs; cycle 1. set_solver. set_solver. set_solver.
+        enough (({[new]} ∪ ∅ : gset nat) = {[new]}). rewrite H; auto. reflexivity. set_solver.
       }
       unfold AuExAny_ra, AuExAnyW_ra, AuExAnyB_ra, maps_to_res. apply pointwise_updatable. i. ur.
       des_ifs; try (rewrite ! URA.unit_id); try (rewrite ! URA.unit_idl); try apply URA.updatable_unit.
@@ -149,139 +131,50 @@ Section Ticket.
       { ii. ur in H. des_ifs. des. ur. split. rewrite URA.unit_id. destruct H. exists x.
         ur in H. des_ifs. ur. auto. ur. auto. }
       { exploit n0. set_solver. intros C; inv C. }
-      ii. auto. }
-    iMod (OwnM_Upd with "TB")  as "[[TB TI] TW]". apply H.
+      ii. auto.
+    }
+    iMod (OwnM_Upd with "TB") as "[[TB TI] TW]". apply H.
     iModIntro. iFrame.
   Qed.
 
-  Lemma Ticket_update r o o' D
+  Lemma Ticket_return γt D old l
     :
-    Ticket_black r o D ∗ Ticket_locked r o ⊢
-      |==> Ticket_black r o' D ∗ Ticket_locked r o'.
+    Ticket_black γt D -∗ Ticket_issued γt old l -∗ Ticket_wait γt old l ==∗ Ticket_black γt (D ∖ {[old]}).
   Proof.
-    iIntros "[TB TL]". unfold Ticket_black, Ticket_locked. iCombine "TB" "TL" as "BL".
-    assert (URA.updatable (Ticket_black_ra r o D ⋅ Ticket_locked_ra r o)
-      (Ticket_black_ra r o' D ⋅ Ticket_locked_ra r o')).
-    { unfold Ticket_black_ra, Ticket_issued_ra. setoid_rewrite maps_to_res_add.
+    iIntros "TB IS WA".
+    unfold Ticket_black, Ticket_issued, Ticket_wait.
+    iCombine "TB" "IS" as "TB". iCombine "TB" "WA" as "TB".
+    assert (URA.updatable (Ticket_black_ra γt D ⋅ Ticket_issued_ra γt old l ⋅ Ticket_wait_ra γt old l)
+      (Ticket_black_ra γt (D ∖ {[old]}))).
+    { unfold Ticket_black_ra, Ticket_issued_ra, Ticket_wait_ra. do 2 setoid_rewrite maps_to_res_add.
       apply maps_to_updatable. ur. apply URA.prod_updatable.
-      { apply Auth.auth_update. ii. des. ur in FRAME.
-        des_ifs. ur in H0. des_ifs. ur in H1. des_ifs. split.
-        { ur. split; ur; auto. }
-        { ur. f_equal. ur; auto. ur; auto. des_ifs. }
-      }
-      ii; auto.
+      ur. rewrite URA.unit_idl. ur. des_ifs. 2:{ set_solver. }
+      ii. ur in H. des_ifs. des. destruct H. ur in H. des_ifs. ur in H. des_ifs.
+      ur. split. exists (Some g0). rewrite URA.unit_idl. ur. des_ifs. 2:{ set_solver. }
+      f_equal. set_solver. ur. auto.
+      unfold AuExAny_ra, AuExAnyW_ra, AuExAnyB_ra, maps_to_res. apply pointwise_updatable. i. ur.
+      des_ifs; try (rewrite ! URA.unit_id); try (rewrite ! URA.unit_idl); try apply URA.updatable_unit.
+      { ur. rewrite URA.unit_id. ii. ur in H. des_ifs. des. ur in H. des_ifs; destruct H; ur in H; des_ifs.
+        ur. split; ur; auto. exists URA.unit. ur. des_ifs. }
+      { exploit n0. set_solver. intros C; inv C. }
+      { ii. ur in H. des_ifs. }
+      { reflexivity. }
     }
-    iMod (OwnM_Upd with "BL") as "BL". apply H. iModIntro. iDestruct "BL" as "[TB TL]". iFrame.
+    iMod (OwnM_Upd with "TB") as "TB". apply H. done.
   Qed.
 
-  Lemma Ticket_issued_wait r tk κu κack κu' κack' :
-    Ticket_issued r tk κu κack ∗ Ticket_wait r tk κu' κack' ⊢ ⌜κu = κu' ∧ κack = κack'⌝.
+  Lemma Ticket_issued_wait γt tk l l' :
+    Ticket_issued γt tk l -∗ Ticket_wait γt tk l' -∗ ⌜l = l'⌝.
   Proof.
-    iIntros "[I W]". unfold Ticket_issued, Ticket_wait, Ticket_issued_ra, Ticket_wait_ra.
+    iIntros "I W". unfold Ticket_issued, Ticket_wait, Ticket_issued_ra, Ticket_wait_ra.
     iCombine "I" "W" as "IW". iPoseProof (OwnM_valid with "IW") as "%IW". setoid_rewrite maps_to_res_add in IW.
-    ur in IW. specialize (IW r). unfold maps_to_res in IW. des_ifs. ur in IW. des.
-    ur in IW0. specialize (IW0 tk). unfold AuExAnyW_ra, AuExAnyB_ra, maps_to_res in IW0. des_ifs.
+    ur in IW. specialize (IW γt). unfold maps_to_res in IW. des_ifs. ur in IW. des.
+    ur in IW0. des. specialize (IW0 tk). unfold AuExAnyW_ra, AuExAnyB_ra, maps_to_res in IW0. des_ifs.
     ur in Heq. inv Heq. inv Heq0. ur in IW0. des_ifs. des. destruct IW0. ur in H. des_ifs.
     apply Any.upcast_inj in H. des. apply JMeq.JMeq_eq in EQ0. inv EQ0. iPureIntro; auto.
   Qed.
 
 End Ticket.
-
-Section Shots.
-  Definition _ShotsRA : URA.t := (nat ==> (URA.prod (OneShot.t nat) (OneShot.t unit)))%ra.
-  Definition ShotsRA : URA.t := (nat ==> _ShotsRA)%ra.
-
-  Context `{Σ : GRA.t}.
-  Context {HasShotsRA : @GRA.inG ShotsRA Σ}.
-
-  Definition ShotsRA_Auth_base : _ShotsRA :=
-    (fun k => (OneShot.pending _ 1, OneShot.pending _ 1)).
-  Definition ShotsRA_Auth : iProp :=
-    (∃ (U : nat), OwnM ((fun k => if (lt_dec k U) then ε else ShotsRA_Auth_base) : ShotsRA)).
-
-  Definition Shots_base_ra sr U : ShotsRA :=
-    maps_to_res sr ((fun k => if (lt_dec k U) then ε else (OneShot.pending _ 1, OneShot.pending _ 1)) : _ShotsRA).
-  Definition Shots_base sr U : iProp := OwnM (Shots_base_ra sr U).
-
-  Definition Shots_pending_ra (sr tk κu : nat) : ShotsRA :=
-    maps_to_res sr (maps_to_res tk ((OneShot.shot κu, OneShot.pending _ 1) : URA.prod _ _)).
-  Definition Shots_pending (sr tk κu : nat) : iProp := OwnM (Shots_pending_ra sr tk κu).
-
-  Definition Shots_shot_ra (sr tk κu : nat) : ShotsRA :=
-    maps_to_res sr (maps_to_res tk ((OneShot.shot κu, OneShot.shot tt) : URA.prod _ _)).
-  Definition Shots_shot (sr tk κu : nat) : iProp := OwnM (Shots_shot_ra sr tk κu).
-
-  Lemma Shots_shot_persistent sr tk κu :
-    Shots_shot sr tk κu ⊢ □ Shots_shot sr tk κu.
-  Proof.
-    iIntros "H". unfold Shots_shot. iPoseProof (own_persistent with "H") as "H".
-    enough (URA.core (Shots_shot_ra sr tk κu) = Shots_shot_ra sr tk κu). rewrite H. done.
-    unfold Shots_shot_ra, maps_to_res. ur. repeat extensionalities. des_ifs.
-    { destruct s; destruct s0; ur; ss. }
-    { destruct s; destruct s0; ur; ss. }
-  Qed.
-
-  Global Program Instance Persistent_Shots_shot sr tk κu : Persistent (Shots_shot sr tk κu).
-  Next Obligation.
-    iIntros (sr tk κu) "S". iApply (Shots_shot_persistent with "S").
-  Qed.
-
-  Lemma ShotsRA_alloc o :
-    ShotsRA_Auth ⊢ ∃ r, |==> ShotsRA_Auth ∗ Shots_base r o.
-  Proof.
-    iIntros "[%U BASE]". iExists U.
-    assert (URA.updatable
-      ((λ k, if lt_dec k U then ε else ShotsRA_Auth_base) : ShotsRA)
-      (((λ k, if lt_dec k (S U) then ε else ShotsRA_Auth_base) : ShotsRA)
-        ⋅ (maps_to_res U ShotsRA_Auth_base))) as UPD.
-    { ur. apply pointwise_updatable. i. unfold maps_to_res. des_ifs; try lia.
-      - rewrite URA.unit_idl. reflexivity.
-      - rewrite URA.unit_idl. reflexivity.
-      - rewrite URA.unit_id. reflexivity.  }
-    iMod (OwnM_Upd with "BASE") as "[A B]". apply UPD.
-    assert (URA.updatable (maps_to_res U ShotsRA_Auth_base) (Shots_base_ra U o)).
-    { unfold ShotsRA_Auth_base, Shots_base_ra, maps_to_res. apply pointwise_updatable. i.
-      des_ifs; cycle 1. apply pointwise_updatable. i. des_ifs. apply URA.updatable_unit. }
-    iMod (OwnM_Upd with "B") as "C". apply H.
-    iModIntro. iSplitL "A".
-    { iExists (S U). auto. }
-    { auto. }
-  Qed.
-
-  Lemma Shots_alloc κu r o : Shots_base r o ⊢ |==> Shots_base r (1 + o) ∗ Shots_pending r o κu.
-  Proof.
-    iIntros "B". unfold Shots_base, Shots_pending.
-    assert (URA.updatable (Shots_base_ra r o) (Shots_base_ra r (1 + o) ⋅ Shots_pending_ra r o κu)).
-    { unfold Shots_base_ra, Shots_pending_ra. setoid_rewrite maps_to_res_add.
-      apply maps_to_updatable. unfold maps_to_res. apply pointwise_updatable. i. ur.
-      des_ifs; try rewrite URA.unit_id; try rewrite URA.unit_idl; try apply URA.updatable_unit;
-        try reflexivity; try lia.
-      apply URA.prod_updatable. apply OneShot.pending_shot. reflexivity. }
-    iMod (OwnM_Upd with "B") as "C". apply H.
-    iModIntro. iDestruct "C" as "[D E]"; iFrame.
-  Qed.
-
-  Lemma Shots_pending_not_shot sr tk κu κu' :
-    Shots_pending sr tk κu ∗ Shots_shot sr tk κu' ⊢ False.
-  Proof.
-    iIntros "[P S]". unfold Shots_pending, Shots_shot. iCombine "P" "S" as "PS".
-    unfold Shots_pending_ra, Shots_shot_ra. iPoseProof (OwnM_valid with "PS") as "%PS".
-    unfold maps_to_res in PS. ur in PS. specialize (PS sr). ur in PS. specialize (PS tk).
-    des_ifs. ur in PS. des. ur in PS0. done.
-  Qed.
-
-  Lemma Shots_pending_shot κu sr tk :
-    Shots_pending sr tk κu ⊢ |==> Shots_shot sr tk κu.
-  Proof.
-    iIntros "P". unfold Shots_pending, Shots_shot.
-    assert (URA.updatable (Shots_pending_ra sr tk κu) (Shots_shot_ra sr tk κu)).
-    {
-      unfold Shots_pending_ra, Shots_shot_ra. do 2 apply maps_to_updatable.
-      apply URA.prod_updatable. reflexivity. apply OneShot.pending_shot.
-    }
-    iMod (OwnM_Upd with "P"). apply H. done.
-  Qed.
-End Shots.
 
 Section SPROP.
 
@@ -291,79 +184,41 @@ Section SPROP.
   Context {TLRAS : TLRAs STT Γ Σ}.
 
   Context {HasTicket : @GRA.inG TicketRA Γ}.
-  Context {HasShots : @GRA.inG ShotsRA Γ}.
+  Context {AuthExclAnys : @GRA.inG (AuthExcls.t (nat * nat * nat))%ra Γ}.
 
   Definition s_ticket_auth {n} : sProp n :=
-    (∃ (U : τ{nat, n}), (➢((fun k => if (lt_dec k U) then ε else TicketRA_Auth_base) : TicketRA)))%S.
+    (∃ (U : τ{nat, n}),
+      (➢((fun k => if (lt_dec k U) then ε else TicketRA_Auth_base) : TicketRA))
+      ∗ SAuthExcls.s_rest (fun k => lt_dec k U) (0, 0, 0))%S.
   Lemma red_s_ticket_auth n :
     ⟦s_ticket_auth, n⟧ = TicketRA_Auth.
   Proof.
     unfold s_ticket_auth, TicketRA_Auth. red_tl; simpl. f_equal. extensionalities r.
-    red_tl. auto.
+    red_tl. red_tl_authexcls. auto.
   Qed.
 
-  Definition s_ticket_black {n} (r o : nat) (D : gset nat) : sProp n :=
-    (➢(Ticket_black_ra r o D))%S.
-  Lemma red_s_ticket_black n r o D :
-    ⟦s_ticket_black r o D, n⟧ = Ticket_black r o D.
+  Definition s_ticket_black {n} (γt : nat) (D : gset nat) : sProp n :=
+    (➢(Ticket_black_ra γt D))%S.
+  Lemma red_s_ticket_black n γt D :
+    ⟦s_ticket_black γt D, n⟧ = Ticket_black γt D.
   Proof.
     unfold s_ticket_black. red_tl; simpl. ss.
   Qed.
 
-  Definition s_ticket_locked {n} (r o : nat) : sProp n :=
-    (➢(Ticket_locked_ra r o))%S.
-  Lemma red_s_ticket_locked n r o :
-    ⟦s_ticket_locked r o, n⟧ = Ticket_locked r o.
-  Proof.
-    unfold s_ticket_locked. red_tl; simpl. ss.
-  Qed.
-
-  Definition s_ticket_issued {n} (r o tid obl : nat) : sProp n :=
-    (➢(Ticket_issued_ra r o tid obl))%S.
-  Lemma red_s_ticket_issued n r o tid obl :
-    ⟦s_ticket_issued r o tid obl, n⟧ = Ticket_issued r o tid obl.
+  Definition s_ticket_issued {n} (γt tk : nat) (l : list nat) : sProp n :=
+    (➢(Ticket_issued_ra γt tk l))%S.
+  Lemma red_s_ticket_issued n γt tk l :
+    ⟦s_ticket_issued γt tk l, n⟧ = Ticket_issued γt tk l.
   Proof.
     unfold s_ticket_issued. red_tl; simpl. ss.
   Qed.
 
-  Definition s_ticket_wait {n} (r o tid obl : nat) : sProp n :=
-    (➢(Ticket_wait_ra r o tid obl))%S.
-  Lemma red_s_ticket_wait n r o tid obl :
-    ⟦s_ticket_wait r o tid obl, n⟧ = Ticket_wait r o tid obl.
+  Definition s_ticket_wait {n} (γt tk : nat) (l : list nat) : sProp n :=
+    (➢(Ticket_wait_ra γt tk l))%S.
+  Lemma red_s_ticket_wait n γt tk l :
+    ⟦s_ticket_wait γt tk l, n⟧ = Ticket_wait γt tk l.
   Proof.
     unfold s_ticket_wait. red_tl; simpl. ss.
-  Qed.
-
-  Definition s_shots_auth {n} : sProp n :=
-    (∃ (U : τ{nat, n}), (➢((fun k => if (lt_dec k U) then ε else ShotsRA_Auth_base) : ShotsRA)))%S.
-  Lemma red_s_shots_auth n :
-    ⟦s_shots_auth, n⟧ = ShotsRA_Auth.
-  Proof.
-    unfold s_shots_auth, ShotsRA_Auth. red_tl; simpl. f_equal. extensionalities r.
-    red_tl. auto.
-  Qed.
-
-  Definition s_shots_base {n} sr U : sProp n :=
-    (➢(Shots_base_ra sr U))%S.
-  Lemma red_s_shots_base sr U n : ⟦s_shots_base sr U, n⟧ = Shots_base sr U.
-  Proof.
-    unfold s_shots_base, Shots_base. red_tl; simpl. f_equal.
-  Qed.
-
-  Definition s_shots_pending {n} (sr tk κu : nat) : sProp n :=
-    (➢(Shots_pending_ra sr tk κu))%S.
-  Lemma red_s_shots_pending n sr tk κu :
-    ⟦s_shots_pending sr tk κu, n⟧ = Shots_pending sr tk κu.
-  Proof.
-    unfold s_shots_pending. red_tl; simpl. ss.
-  Qed.
-
-  Definition s_shots_shot {n} (sr tk κu : nat) : sProp n :=
-    (➢(Shots_shot_ra sr tk κu))%S.
-  Lemma red_s_shots_shot n sr tk κu :
-    ⟦s_shots_shot sr tk κu, n⟧ = Shots_shot sr tk κu.
-  Proof.
-    unfold s_shots_shot. red_tl; simpl. ss.
   Qed.
 
 End SPROP.
@@ -371,21 +226,11 @@ End SPROP.
 Ltac red_tl_ticket := (try rewrite ! red_s_ticket_auth;
                        try rewrite ! red_s_ticket_black;
                        try rewrite ! red_s_ticket_issued;
-                       try rewrite ! red_s_ticket_locked;
-                       try rewrite ! red_s_ticket_wait;
-                       try rewrite ! red_s_shots_auth;
-                       try rewrite ! red_s_shots_base;
-                       try rewrite ! red_s_shots_pending;
-                       try rewrite ! red_s_shots_shot
+                       try rewrite ! red_s_ticket_wait
                       ).
 
 Ltac red_tl_lifetime_s := (try setoid_rewrite red_s_ticket_auth;
                            try setoid_rewrite red_s_ticket_black;
                            try setoid_rewrite red_s_ticket_issued;
-                           try setoid_rewrite red_s_ticket_locked;
-                           try setoid_rewrite red_s_ticket_wait;
-                           try setoid_rewrite red_s_shots_base;
-                           try setoid_rewrite red_s_shots_auth;
-                           try setoid_rewrite red_s_shots_pending;
-                           try setoid_rewrite red_s_shots_shot
+                           try setoid_rewrite red_s_ticket_wait
                           ).
